src/SoftBound/sb_ds_pp.v
@@ -1,31 +1,2990 @@
 Add LoadPath "../ssa/ott".
 Add LoadPath "../ssa/monads".
-Add LoadPath "../ssa/compcert".
 Add LoadPath "../ssa".
+Add LoadPath "../ssa/compcert".
 Add LoadPath "../../../theory/metatheory_8.3".
 Add LoadPath "../TV".
 Require Import ssa_def.
 Require Import ssa_lib.
 Require Import List.
-Require Export targetdata.
-Require Import monad.
 Require Import Arith.
+Require Import tactics.
+Require Import monad.
+Require Import trace.
 Require Import Metatheory.
 Require Import genericvalues.
-Require Import trace.
-Require Import ssa_props.
 Require Import alist.
-Require Import sb_def.
-Require Import Coqlib.
-Require Import Memdata.
+Require Import Values.
 Require Import Memory.
 Require Import Integers.
-Require Import sb_tactic.
-Require Import symexe_def.
-Require Import symexe_tactic.
-Require Import Znumtheory.
-Require Import sb_metadata.
+Require Import Coqlib.
+Require Import targetdata.
+Require Import Maps.
+Require Import Lattice.
+Require Import Iteration.
+Require Import Kildall.
+Require Import ssa_static.
+Require Import ssa_props.
+Require Import ssa_analysis.
+Require Import ssa_wf.
 Require Import ssa_dynamic.
+Require Import sb_ds_def.
+Require Import sbop_dsop.
+
+Export LLVMwf.
+Export AtomSet.
+Export LLVMgv.
+Export SBopsem.
+
+Definition wf_rmap (f:fdef) (lc:GVMap) (rm:rmetadata) : Prop :=
+forall id1 gv1 t1, 
+  lookupAL _ lc id1 = Some gv1 -> 
+  lookupTypViaIDFromFdef f id1 = Some (typ_pointer t1) ->
+  exists md, lookupAL _ rm id1 = Some md.
+
+Definition wf_ExecutionContext (ps:list product) (ec:SBopsem.ExecutionContext) 
+  : Prop :=
+let '(SBopsem.mkEC f b cs tmn lc rm als) := ec in
+isReachableFromEntry f b /\
+blockInFdefB b f = true /\
+InProductsB (product_fdef f) ps = true /\
+match cs with
+| nil => 
+    match inscope_of_tmn f b tmn with
+    | Some ids => wf_defs f lc ids
+    | None => False
+    end
+| c::_ =>
+    match inscope_of_cmd f b c with
+    | Some ids => wf_defs f lc ids
+    | None => False
+    end
+end /\
+wf_rmap f lc rm /\
+exists l1, exists ps, exists cs',
+b = block_intro l1 ps (cs'++cs) tmn.
+
+Definition wf_call (ec:SBopsem.ExecutionContext) (ecs:SBopsem.ECStack) 
+  : Prop :=
+let '(SBopsem.mkEC f _ _ _ _ _ _) := ec in
+forall b, blockInFdefB b f ->
+let '(block_intro _ _ _ tmn) := b in
+match tmn with
+| insn_return _ _ _ | insn_return_void _ =>
+    match ecs with
+    | nil => True
+    | SBopsem.mkEC f' b' (insn_call _ _ _ _ _ _ ::_) tmn' lc' rm' als'::ecs' =>
+        True
+    | _ => False
+    end
+| _ => True
+end.
+
+Fixpoint wf_ECStack (ps:list product) (ecs:SBopsem.ECStack) : Prop :=
+match ecs with
+| nil => False
+| ec::ecs' => wf_ExecutionContext ps ec /\ wf_ECStack ps ecs' /\ wf_call ec ecs'
+end.
+
+Definition wf_State (S:SBopsem.State) : Prop :=
+let '(SBopsem.mkState s (los, nts) ps ecs gl _ _ _) := S in
+wf_global s gl /\
+wf_system nil s /\
+moduleInSystemB (module_intro los nts ps) s = true /\
+wf_ECStack ps ecs.
+
+(*********************************************)
+(** * Preservation *)
+
+Definition preserved_MM (MM MM':SBopsem.mmetadata) := True.
+
+Hint Unfold preserved_MM.
+
+Lemma preservation_cmd_updated_case : forall
+  (S : system)
+  (los : layouts)
+  (nts : namedts)
+  (Ps : list product)
+  (F : fdef)
+  (B : block)
+  (lc : GVMap)
+  (gl : GVMap)
+  (fs : GVMap)
+  (gv3 : GenericValue)
+  (EC : list SBopsem.ExecutionContext)
+  (cs : list cmd)
+  (tmn : terminator)
+  (Mem0 : mem)
+  (als : list mblock)
+  id0 c0
+  (Hid : Some id0 = getCmdID c0)
+  t0
+  (Htyp : Some t0 = getCmdTyp c0)
+  MM rm rm'
+  (Hprm : wf_rmap F lc rm -> wf_rmap F (updateAddAL GenericValue lc id0 gv3) rm')
+  (HwfS1 : wf_State
+            {|
+            SBopsem.CurSystem := S;
+            SBopsem.CurTargetData := (los, nts);
+            SBopsem.CurProducts := Ps;
+            SBopsem.ECS := {|
+                   SBopsem.CurFunction := F;
+                   SBopsem.CurBB := B;
+                   SBopsem.CurCmds := c0 :: cs;
+                   SBopsem.Terminator := tmn;
+                   SBopsem.Locals := lc;
+                   SBopsem.Rmap := rm;
+                   SBopsem.Allocas := als |} :: EC;
+            SBopsem.Globals := gl;
+            SBopsem.FunTable := fs;
+            SBopsem.Mem := Mem0;
+            SBopsem.Mmap := MM |}),
+   wf_State
+     {|
+     SBopsem.CurSystem := S;
+     SBopsem.CurTargetData := (los, nts);
+     SBopsem.CurProducts := Ps;
+     SBopsem.ECS := {|
+            SBopsem.CurFunction := F;
+            SBopsem.CurBB := B;
+            SBopsem.CurCmds := cs;
+            SBopsem.Terminator := tmn;
+            SBopsem.Locals := updateAddAL GenericValue lc id0 gv3;
+            SBopsem.Rmap := rm';
+            SBopsem.Allocas := als |} :: EC;
+     SBopsem.Globals := gl;
+     SBopsem.FunTable := fs;
+     SBopsem.Mem := Mem0;
+     SBopsem.Mmap := MM |}.
+Proof.
+  intros.
+  destruct HwfS1 as 
+    [Hwfg [HwfSystem [HmInS [
+     [Hreach1 [HBinF1 [HFinPs1 [Hinscope1 [Hwfm [l3 [ps3 [cs3' Heq1]]]]]]]]
+     [HwfEC HwfCall]]]]
+    ]; subst.
+  remember (inscope_of_cmd F (block_intro l3 ps3 (cs3' ++ c0 :: cs) tmn) c0) 
+    as R1. 
+  destruct R1; try solve [inversion Hinscope1].
+  repeat (split; try solve [auto]).
+      assert (Hid':=Hid).
+      symmetry in Hid.
+      apply getCmdLoc_getCmdID in Hid.
+       subst.
+      destruct cs; simpl_env in *.
+      Case "1.1.1".
+        assert (~ In (getCmdLoc c0) (getCmdsLocs cs3')) as Hnotin.
+          eapply wf_system__uniq_block with (f:=F) in HwfSystem; eauto.        
+          simpl in HwfSystem.
+          apply NoDup_inv in HwfSystem.
+          destruct HwfSystem as [_ J].
+          apply NoDup_inv in J.
+          destruct J as [J _].
+          rewrite getCmdsLocs_app in J.
+          simpl in J.
+          apply NoDup_last_inv in J. auto.
+
+        apply inscope_of_cmd_tmn in HeqR1; auto.
+        destruct HeqR1 as [ids2 [J1 J2]].        
+        rewrite <- J1.
+        assert (In c0 (cs3' ++ [c0])) as HinCs.
+          apply in_or_app. right. simpl. auto.
+        assert (Hwfc := HBinF1).
+        eapply wf_system__wf_cmd with (c:=c0) in Hwfc; 
+          eauto.
+        rewrite <- Hid' in J2.
+        eapply wf_defs_updateAddAL with (t1:=t0) ; eauto.
+          eapply uniqF__lookupTypViaIDFromFdef; eauto.
+            eapply wf_system__uniqFdef; eauto.
+        
+      Case "1.1.2".
+        assert (NoDup (getCmdsLocs (cs3' ++ [c0] ++ [c] ++ cs))) as Hnodup.
+          eapply wf_system__uniq_block with (f:=F) in HwfSystem; eauto.        
+          simpl in HwfSystem.
+          apply NoDup_inv in HwfSystem.
+          destruct HwfSystem as [_ J].
+          apply NoDup_inv in J.
+          destruct J as [J _]. auto.
+        apply inscope_of_cmd_cmd in HeqR1; auto.
+        destruct HeqR1 as [ids2 [J1 J2]].        
+        rewrite <- J1.
+        assert (In c0 (cs3' ++ [c0] ++ [c] ++ cs)) as HinCs.
+          apply in_or_app. right. simpl. auto.
+        assert (Hwfc := HBinF1).
+        eapply wf_system__wf_cmd with (c:=c0) in Hwfc; 
+          eauto.
+        rewrite <- Hid' in J2.
+        eapply wf_defs_updateAddAL with (t1:=t0) ; eauto.
+          eapply uniqF__lookupTypViaIDFromFdef; eauto.
+            eapply wf_system__uniqFdef; eauto.
+
+  exists l3. exists ps3. exists (cs3'++[c0]). simpl_env. auto.
+Qed.
+
+Lemma preservation_cmd_non_updated_case : forall
+  (S : system)
+  (los : layouts)
+  (nts : namedts)
+  (Ps : list product)
+  (F : fdef)
+  (B : block)
+  (lc : GVMap)
+  (gl : GVMap)
+  (fs : GVMap)
+  (EC : list SBopsem.ExecutionContext)
+  (cs : list cmd)
+  (tmn : terminator)
+  (Mem0 : mem)
+  (als : list mblock)
+  c0
+  (Hid : getCmdID c0 = None)
+  rm MM MM'
+  (HpMM : preserved_MM MM MM')
+  (HwfS1 : wf_State
+            {|
+            SBopsem.CurSystem := S;
+            SBopsem.CurTargetData := (los, nts);
+            SBopsem.CurProducts := Ps;
+            SBopsem.ECS := {|
+                   SBopsem.CurFunction := F;
+                   SBopsem.CurBB := B;
+                   SBopsem.CurCmds := c0 :: cs;
+                   SBopsem.Terminator := tmn;
+                   SBopsem.Locals := lc;
+                   SBopsem.Rmap := rm;
+                   SBopsem.Allocas := als |} :: EC;
+            SBopsem.Globals := gl;
+            SBopsem.FunTable := fs;
+            SBopsem.Mem := Mem0;
+            SBopsem.Mmap := MM |}),
+   wf_State
+     {|
+     SBopsem.CurSystem := S;
+     SBopsem.CurTargetData := (los, nts);
+     SBopsem.CurProducts := Ps;
+     SBopsem.ECS := {|
+            SBopsem.CurFunction := F;
+            SBopsem.CurBB := B;
+            SBopsem.CurCmds := cs;
+            SBopsem.Terminator := tmn;
+            SBopsem.Locals := lc;
+            SBopsem.Rmap := rm;
+            SBopsem.Allocas := als |} :: EC;
+     SBopsem.Globals := gl;
+     SBopsem.FunTable := fs;
+     SBopsem.Mem := Mem0;
+     SBopsem.Mmap := MM' |}.
+Proof.
+  intros.
+  destruct HwfS1 as 
+    [Hwfg [HwfSystem [HmInS [
+     [Hreach1 [HBinF1 [HFinPs1 [Hinscope1 [Hwfm [l3 [ps3 [cs3' Heq1]]]]]]]]
+     [HwfEC HwfCall]]]]
+    ]; subst.
+  remember (inscope_of_cmd F (block_intro l3 ps3 (cs3' ++ c0 :: cs) tmn) c0) 
+    as R1. 
+  destruct R1; try solve [inversion Hinscope1].
+  repeat (split; try solve [auto]).
+      destruct cs; simpl_env in *.
+      Case "1.1.1".
+        assert (~ In (getCmdLoc c0) (getCmdsLocs cs3')) as Hnotin.
+          eapply wf_system__uniq_block with (f:=F) in HwfSystem; eauto.        
+          simpl in HwfSystem.
+          apply NoDup_inv in HwfSystem.
+          destruct HwfSystem as [_ J].
+          apply NoDup_inv in J.
+          destruct J as [J _].
+          rewrite getCmdsLocs_app in J.
+          simpl in J.
+          apply NoDup_last_inv in J. auto.
+
+        apply inscope_of_cmd_tmn in HeqR1; auto.
+        destruct HeqR1 as [ids2 [J1 J2]].        
+        rewrite <- J1.
+        assert (In c0 (cs3' ++ [c0])) as HinCs.
+          apply in_or_app. right. simpl. auto.
+        assert (Hwfc := HBinF1).
+        eapply wf_system__wf_cmd with (c:=c0) in Hwfc; 
+          eauto.
+        rewrite Hid in J2.
+        eapply wf_defs_eq; eauto.
+        
+      Case "1.1.2".
+        assert (NoDup (getCmdsLocs (cs3' ++ [c0] ++ [c] ++ cs))) as Hnodup.
+          eapply wf_system__uniq_block with (f:=F) in HwfSystem; eauto.        
+          simpl in HwfSystem.
+          apply NoDup_inv in HwfSystem.
+          destruct HwfSystem as [_ J].
+          apply NoDup_inv in J.
+          destruct J as [J _]. auto.
+        apply inscope_of_cmd_cmd in HeqR1; auto.
+        destruct HeqR1 as [ids2 [J1 J2]].        
+        rewrite <- J1.
+        assert (In c0 (cs3' ++ [c0] ++ [c] ++ cs)) as HinCs.
+          apply in_or_app. right. simpl. auto.
+        assert (Hwfc := HBinF1).
+        eapply wf_system__wf_cmd with (c:=c0) in Hwfc; 
+          eauto.
+        rewrite Hid in J2.
+        eapply wf_defs_eq ; eauto.
+
+  exists l3. exists ps3. exists (cs3'++[c0]). simpl_env. auto.
+Qed.
+
+Lemma returnUpdateLocals__wf_rmap : 
+  forall los nts Mem' c' Result lc lc' rm rm' gl lc'' rm'' F' tmn' cs' Ps S
+  (H1 : returnUpdateLocals (los, nts) Mem' c' Result lc lc' rm rm' gl =
+       ret (lc'', rm''))
+  (HwfSystem : wf_system nil S)
+  (HmInS : moduleInSystemB (module_intro los nts Ps) S = true)
+  (HFinPs2 : InProductsB (product_fdef F') Ps = true)
+  (Hwfm2 : wf_rmap F' lc' rm')
+  (l2 : l)
+  (ps2 : phinodes)
+  (cs2' : list cmd) 
+  (HBinF2 : blockInFdefB (block_intro l2 ps2 (cs2' ++ c' :: cs') tmn') F' =
+           true)
+  (Hwfc : wf_insn nil S (module_intro los nts Ps) F'
+           (block_intro l2 ps2 (cs2' ++ c' :: cs') tmn') 
+           (insn_cmd c')),
+  wf_rmap F' lc'' rm''.
+Proof.
+  intros.
+      eapply wf_system__uniqFdef with (f:=F') in HwfSystem; eauto.
+      unfold returnUpdateLocals in H1.
+      destruct c'; inv H1; auto.
+      destruct n; inv H0; auto.
+      remember (getOperandValue (los, nts) Mem' Result lc gl) as R1.
+      destruct R1; inv H1.
+      inv Hwfc. 
+      clear H12 H17 H6 H15 H16.
+      assert (lookupTypViaIDFromFdef F' i0 = Some typ1) as J.
+        eapply uniqF__lookupTypViaIDFromFdef with 
+          (c:=insn_call i0 false c
+                   (typ_function typ1
+                      (make_list_typ
+                         (map_list_typ_value
+                            (fun (typ_' : typ) (_ : value) => typ_')
+                            typ'_value''_list)) varg5) v
+                   (map_list_typ_value
+                      (fun (typ_' : typ) (value_'' : value) =>
+                       (typ_', value_'')) typ'_value''_list))(i0:=i0)(t0:=typ1)
+          in HBinF2; eauto.
+          apply in_or_app. right. simpl. auto.
+      clear HBinF2.
+      intros x gvx tx Hin Htyp.
+      destruct (eq_atom_dec x i0); subst.        
+        rewrite J in Htyp. inv Htyp.
+        remember (get_reg_metadata (los, nts) Mem' gl rm Result) as R3.
+        destruct R3 as [[md ?]|]; inv H0.
+          rewrite lookupAL_updateAddAL_eq. eauto.
+          rewrite lookupAL_updateAddAL_eq. eauto.
+       
+        destruct typ1; inv H0; try solve [
+          rewrite <- lookupAL_updateAddAL_neq in Hin; auto;
+          eapply Hwfm2 in Hin; eauto
+        ].
+          destruct (get_reg_metadata (los, nts) Mem' gl rm Result)
+            as [[md ?]|]; inv H1; try solve [
+            rewrite <- lookupAL_updateAddAL_neq in Hin; auto;
+            rewrite <- lookupAL_updateAddAL_neq; eauto
+          ].
+Qed.
+
+Lemma getIncomingValuesForBlockFromPHINodes_spec : forall ps TD Mem0 b gl lc id1
+    rm re gv1 opmd1,
+  Some re = getIncomingValuesForBlockFromPHINodes TD Mem0 ps b gl lc rm ->
+  In (id1, gv1, opmd1) re ->
+  In id1 (getPhiNodesIDs ps).
+Proof.    
+  induction ps; intros; simpl in *.
+    inv H. inversion H0.
+
+    destruct a.
+    destruct (getValueViaBlockFromValuels l0 b); try solve [inversion H].   
+    destruct (getOperandValue TD Mem0 v lc gl); try solve [inversion H].   
+    remember (getIncomingValuesForBlockFromPHINodes TD Mem0 ps b gl lc rm) as R.
+    destruct R; try solve [inv H].
+    simpl.
+    destruct (isPointerTypB t); inv H.
+      destruct (get_reg_metadata TD Mem0 gl rm v) as [[md mt]|]; inv H2.      
+      simpl in H0.
+      destruct H0 as [H0 | H0]; eauto.  
+        inv H0; auto.
+
+      simpl in H0.
+      destruct H0 as [H0 | H0]; eauto.  
+        inv H0; auto.
+Qed.
+
+Lemma getIncomingValuesForBlockFromPHINodes__wf_rmap : forall PNs TD M b gl lc rm
+   re id1 gv1 opmd1 t1,
+  NoDup (getPhiNodesIDs PNs) ->
+  getIncomingValuesForBlockFromPHINodes TD M PNs b gl lc rm = Some re ->
+  In (id1,gv1,opmd1) re ->
+  lookupTypViaIDFromPhiNodes PNs id1 = Some (typ_pointer t1) ->
+  opmd1 <> None.
+Proof.
+  induction PNs; simpl; intros TD M b gl lc rm re id1 gv1 opmd1 t1 Huniq Hget Hin
+    Hlk.
+    inv Hget. inversion Hin.
+
+    inv Huniq.
+    destruct a.
+    destruct (getValueViaBlockFromValuels l0 b); try solve [inv Hget].
+    destruct (getOperandValue TD M v lc gl); try solve [inv Hget].    
+    remember (getIncomingValuesForBlockFromPHINodes TD M PNs b gl lc rm) as R.
+    destruct R; try solve [inv Hget].
+    unfold lookupTypViaIDFromPhiNode in Hlk. simpl in Hlk.
+    destruct (id1==i0); subst.
+      inv Hlk.
+      simpl in Hget.
+      remember (get_reg_metadata TD M gl rm v) as R.
+      destruct R as [[md mt]|]; inv Hget.
+      simpl in Hin.
+      destruct Hin as [Hin | Hin]; try (inv Hin; congruence).
+        simpl in H1.         
+        eapply getIncomingValuesForBlockFromPHINodes_spec in HeqR; eauto.
+
+      destruct (isPointerTypB t); inv Hget.
+        destruct (get_reg_metadata TD M gl rm v) as [[md mt]|]; inv H0.
+        simpl in Hin.
+        destruct Hin as [Hin | Hin].
+          inv Hin. congruence.
+          eauto.
+        simpl in Hin.
+        destruct Hin as [Hin | Hin].
+          inv Hin. congruence.
+          eauto.
+Qed.
+
+Lemma updateValuesForNewBlock_spec1 : forall rvs lc x rm lc' rm' gv,
+  lookupAL _ lc x = None ->
+  (lc', rm') = updateValuesForNewBlock rvs lc rm ->
+  lookupAL _ lc' x = Some gv ->
+  exists omd, In (x, gv, omd) rvs.
+Proof.
+  induction rvs; simpl; intros lc x rm lc' rm' gv Hlk Hupdate Hlk'.
+    inv Hupdate. rewrite Hlk in Hlk'. inversion Hlk'.
+
+    destruct a. destruct p.
+    remember (updateValuesForNewBlock rvs lc rm) as R.
+    destruct R as [lc1 rm1].
+    destruct o as [[md ?]|]; inv Hupdate.
+      destruct (eq_atom_dec i0 x); subst.
+        rewrite lookupAL_updateAddAL_eq in Hlk'; auto.
+        inv Hlk'. eauto.
+
+        rewrite <- lookupAL_updateAddAL_neq in Hlk'; auto.
+        eapply IHrvs in HeqR; eauto.
+        destruct HeqR as [omd HeqR]. eauto.
+
+      destruct (eq_atom_dec i0 x); subst.
+        rewrite lookupAL_updateAddAL_eq in Hlk'; auto.
+        inv Hlk'. eauto.
+
+        rewrite <- lookupAL_updateAddAL_neq in Hlk'; auto.
+        eapply IHrvs in HeqR; eauto.
+        destruct HeqR as [omd HeqR]. eauto.
+Qed.
+
+Lemma updateValuesForNewBlock_spec2 : forall rvs lc x rm lc' rm' md,
+  lookupAL _ rm x = Some md ->
+  (lc', rm') = updateValuesForNewBlock rvs lc rm ->
+  exists md, lookupAL _ rm' x = Some md.
+Proof.
+  induction rvs; simpl; intros lc x rm lc' rm' md Hlk Hupdate.
+    inv Hupdate; eauto.
+
+    destruct a. destruct p.
+    remember (updateValuesForNewBlock rvs lc rm) as R.
+    destruct R as [lc1 rm1].
+    destruct o as [[md1 ?]|]; inv Hupdate.
+      destruct (eq_atom_dec i0 x); subst.
+        rewrite lookupAL_updateAddAL_eq.
+        eauto.
+
+        rewrite <- lookupAL_updateAddAL_neq; auto.
+        eapply IHrvs in HeqR; eauto.
+
+      eapply IHrvs in HeqR; eauto.
+Qed.
+
+Lemma updateValuesForNewBlock_spec3 : forall rvs lc x rm lc' rm' gvx md mt,
+  In (x, gvx, Some (md,mt)) rvs ->
+  (lc', rm') = updateValuesForNewBlock rvs lc rm ->
+  exists md, lookupAL _ rm' x = Some md.
+Proof.
+  induction rvs; simpl; intros lc x rm lc' rm' gvx md mt Hin Hupdate.
+    inversion Hin.
+
+    destruct a. destruct p.
+    remember (updateValuesForNewBlock rvs lc rm) as R.
+    destruct R as [lc1 rm1].
+    destruct o as [[md1 ?]|]; inv Hupdate.
+      destruct (eq_atom_dec i0 x); subst.
+        rewrite lookupAL_updateAddAL_eq. eauto.
+
+        rewrite <- lookupAL_updateAddAL_neq; auto.
+        destruct Hin as [Hin | Hin].
+          inv Hin. contradict n; auto.
+          eapply IHrvs in HeqR; eauto.
+
+      destruct Hin as [Hin | Hin].
+        inv Hin. 
+        eapply IHrvs in HeqR; eauto.
+Qed.
+
+Lemma updateValuesForNewBlock__wf_rmap_aux : forall rvs F rm lc,
+  (forall id1 gv1 opmd1 t1, 
+    In (id1,gv1,opmd1) rvs ->
+    lookupTypViaIDFromFdef F id1 = Some (typ_pointer t1) ->
+    opmd1 <> None) ->
+  forall rvs2 rvs1 lc1 rm1 lc2 rm2,
+  rvs = rvs1 ++ rvs2 ->
+  updateValuesForNewBlock rvs1 lc rm = (lc1, rm1) ->
+  wf_rmap F lc1 rm1 ->
+  updateValuesForNewBlock rvs2 lc1 rm1 = (lc2, rm2) ->
+  wf_rmap F lc2 rm2.
+Proof.
+  intros rvs F rm lc Hprop.
+  induction rvs2; simpl; intros rvs1 lc1 rm1 lc2 rm2 Heq Hupdate1 Hrmap1
+    Hupdate2; subst.
+    inv Hupdate2. auto.
+
+    destruct a. destruct p.
+    remember (updateValuesForNewBlock rvs2 lc1 rm1) as R. 
+    destruct R as [lc2' rm2'].
+    destruct o as [[md ?]|]; inv Hupdate2.
+      intros x gvx tx Hlk Htyp.
+      destruct (eq_atom_dec i0 x); subst.
+        rewrite lookupAL_updateAddAL_eq. eauto.
+
+        rewrite <- lookupAL_updateAddAL_neq; auto.
+        rewrite <- lookupAL_updateAddAL_neq in Hlk; auto.
+        remember (lookupAL _ lc1 x) as R.
+        destruct R as [gv|].
+          symmetry in HeqR0.
+          assert (exists md0, lookupAL metadata rm1 x = ret md0) as J.
+            eapply Hrmap1; eauto.
+          destruct J as [md0 J].
+          eapply updateValuesForNewBlock_spec2 in J; eauto.
+
+          symmetry in HeqR0.
+          eapply updateValuesForNewBlock_spec1 in HeqR0; eauto.
+          destruct HeqR0 as [omd HeqR0].
+          apply Hprop with (gv1:=gvx)(opmd1:=omd) in Htyp; eauto.
+            destruct omd as [[md1 mt1]|]; try solve [contradict Htyp; auto].
+            eapply updateValuesForNewBlock_spec3 in HeqR; eauto.
+
+            apply in_or_app. simpl. auto.
+
+      intros x gvx tx Hlk Htyp.
+      destruct (eq_atom_dec i0 x); subst.
+        rewrite lookupAL_updateAddAL_eq in Hlk. inv Hlk.
+        apply Hprop with (gv1:=gvx)(opmd1:=merror) in Htyp; auto.
+          contradict Htyp; auto.
+          apply in_or_app. simpl. auto.
+         
+        rewrite <- lookupAL_updateAddAL_neq in Hlk; auto.
+        remember (lookupAL _ lc1 x) as R.
+        destruct R as [gv|].
+          symmetry in HeqR0.
+          assert (exists md0, lookupAL metadata rm1 x = ret md0) as J.
+            eapply Hrmap1; eauto.
+          destruct J as [md0 J].
+          eapply updateValuesForNewBlock_spec2 in J; eauto.
+
+          symmetry in HeqR0.
+          eapply updateValuesForNewBlock_spec1 in HeqR0; eauto.
+          destruct HeqR0 as [omd HeqR0].
+          eapply Hprop with (gv1:=gvx)(opmd1:=omd) in Htyp; eauto.
+            destruct omd as [[md1 mt1]|]; try solve [contradict Htyp; auto].
+            eapply updateValuesForNewBlock_spec3 in HeqR; eauto.
+
+            apply in_or_app. simpl. auto.
+Qed.
+
+Lemma updateValuesForNewBlock__wf_rmap : forall rvs F lc rm lc' rm',
+  wf_rmap F lc rm ->
+  (forall id1 gv1 opmd1 t1, 
+    In (id1,gv1,opmd1) rvs ->
+    lookupTypViaIDFromFdef F id1 = Some (typ_pointer t1) ->
+    opmd1 <> None) ->
+  updateValuesForNewBlock rvs lc rm = (lc', rm') ->
+  wf_rmap F lc' rm'.
+Proof.
+  intros.
+  eapply updateValuesForNewBlock__wf_rmap_aux with (rvs1:=nil)(lc1:=lc)(rm1:=rm)
+    (rvs2:=rvs); simpl; eauto.
+Qed.
+
+Lemma lookupTypViaIDFromFdef__lookupTypViaIDFromPhiNodes : forall F id1 t b1,
+  uniqFdef F ->
+  lookupTypViaIDFromFdef F id1 = Some t ->
+  blockInFdefB b1 F ->
+  In id1 (getPhiNodesIDs (getPHINodesFromBlock b1)) ->
+  lookupTypViaIDFromPhiNodes (getPHINodesFromBlock b1) id1 = Some t. 
+Admitted.
+
+Lemma uniqFdef__uniqBlock : forall F b1,
+  uniqFdef F -> blockInFdefB b1 F -> NoDup (getBlockLocs b1).
+Proof.
+  intros.
+  destruct F. destruct f.
+  destruct H as [H _]. simpl in H0. destruct H.
+  apply NoDup__InBlocksB in H0; auto.
+Qed.
+
+Lemma switchToNewBasicBlock__wf_rmap : forall F TD M b1 b2 gl lc rm lc' rm',
+  uniqFdef F ->
+  blockInFdefB b1 F ->
+  wf_rmap F lc rm ->
+  switchToNewBasicBlock TD M b1 b2 gl lc rm = Some (lc', rm') ->
+  wf_rmap F lc' rm'.
+Proof.
+  intros F TD M b1 b2 gl lc rm lc' rm' Huniq HBinF Hwfm Hswitch.
+  unfold switchToNewBasicBlock in Hswitch.
+  remember (getIncomingValuesForBlockFromPHINodes TD M 
+             (getPHINodesFromBlock b1) b2 gl lc rm) as R.
+  destruct R; inv Hswitch.
+  eapply updateValuesForNewBlock__wf_rmap; eauto.
+  intros.
+  eapply getIncomingValuesForBlockFromPHINodes__wf_rmap with (t1:=t1); eauto.
+    apply uniqFdef__uniqBlock in HBinF; auto.
+    destruct b1. simpl in HBinF. simpl.
+    apply NoDup_inv in HBinF. destruct HBinF; auto.
+
+    eapply lookupTypViaIDFromFdef__lookupTypViaIDFromPhiNodes; eauto.
+      eapply getIncomingValuesForBlockFromPHINodes_spec; eauto.
+Qed.
+
+Lemma updateAddAL_nptr__wf_rmap : forall F lc rm id0 gv3,
+  wf_rmap F lc rm -> 
+  (forall t0, lookupTypViaIDFromFdef F id0 <> Some (typ_pointer t0)) ->
+  wf_rmap F (updateAddAL GenericValue lc id0 gv3) rm.
+Proof.
+  intros.
+  intros x gv t J1 J2.
+  destruct (eq_atom_dec id0 x); subst.
+    contradict J2; auto.
+
+    rewrite <- lookupAL_updateAddAL_neq in J1; eauto.
+Qed.
+
+Lemma updateAddAL_ptr__wf_rmap: forall F lc rm id0 gv3 md,
+  wf_rmap F lc rm -> 
+  wf_rmap F (updateAddAL GenericValue lc id0 gv3) (updateAddAL _ rm id0 md).
+Proof.
+  intros.
+  intros x gv t J1 J2.
+  destruct (eq_atom_dec id0 x); subst.
+    rewrite lookupAL_updateAddAL_eq in J1.
+    rewrite lookupAL_updateAddAL_eq.
+    inv J1. eauto.
+
+    rewrite <- lookupAL_updateAddAL_neq in J1; auto.
+    rewrite <- lookupAL_updateAddAL_neq; eauto. 
+Qed.
+
+Lemma initLocals__wf_rmap : forall ogvs rm lc' rm' fa rt fid la va lb lp TD
+    Mem0 gl lc,
+  params2GVs TD Mem0 lp lc gl rm = ret ogvs ->
+  initLocals la ogvs rm = (lc', rm') ->
+  wf_rmap (fdef_intro (fheader_intro fa rt fid la va) lb) lc' rm'.
+Admitted.
+
+Lemma wf_State__cmd__lookupTypViaIDFromFdef : forall S,
+  wf_State S ->
+  match S with 
+  | {| ECS := {|CurFunction := F; CurCmds := c :: cs |} :: EC |} =>
+      forall id0, getCmdID c = Some id0 ->
+      lookupTypViaIDFromFdef F id0 = getCmdTyp c
+  | _ => True
+  end.
+Admitted.
+
+Ltac preservation_tac HwfS1 :=
+  eapply preservation_cmd_updated_case in HwfS1; simpl; try solve [
+      eauto | 
+      intro J;
+      apply updateAddAL_nptr__wf_rmap; try solve [auto |
+        apply wf_State__cmd__lookupTypViaIDFromFdef in HwfS1;
+        rewrite HwfS1; simpl; try solve [auto | congruence]]
+    ].
+
+Lemma wf_State__wf_cmd : forall St,
+  wf_State St ->
+  match St with 
+  | {| CurSystem := sys;
+       CurTargetData := (los, nts);
+       CurProducts := Ps;
+       ECS := {|CurFunction := F; CurBB := B; CurCmds := c :: cs |} :: EC 
+     |} => wf_insn nil sys (module_intro los nts Ps) F B (insn_cmd c)
+  | _ => True
+  end.
+Admitted.
+
+Lemma preservation : forall S1 S2 tr,
+  SBopsem.dsInsn S1 S2 tr -> wf_State S1 -> wf_State S2.
+Proof.
+  intros S1 S2 tr HdsInsn HwfS1.
+  (sb_dsInsn_cases (induction HdsInsn) Case); destruct TD as [los nts];
+    try invert_prop_reg_metadata.
+Focus.
+Case "dsReturn".
+  destruct HwfS1 as 
+    [Hwfg [HwfSystem [HmInS [
+     [Hreach1 [HBinF1 [HFinPs1 [Hinscope1 [Hwfm1 [l1 [ps1 [cs1' Heq1]]]]]]]] 
+     [
+       [
+         [Hreach2 [HBinF2 [HFinPs2 [Hinscope2 [Hwfm2 [l2 [ps2 [cs2' Heq2]]]]]]]]
+         [HwfEC HwfCall]
+       ]
+       HwfCall'
+     ]
+    ]]]]; subst.
+  remember (inscope_of_cmd F' (block_intro l2 ps2 (cs2' ++ c' :: cs') tmn') c')
+    as R2.
+  destruct R2; try solve [inversion Hinscope2].
+  remember (inscope_of_tmn F
+             (block_intro l1 ps1 (cs1' ++ nil)(insn_return rid RetTy Result))
+             (insn_return rid RetTy Result)) as R1. 
+  destruct R1; try solve [inversion Hinscope1].
+  split; auto.
+  split; auto.
+  SCase "1".
+    split; auto.
+    split; auto.  
+    split; auto. 
+    split; auto.
+    split; auto.
+    assert (Hwfc := HBinF2).
+    assert (In c' (cs2'++[c']++cs')) as HinCs.
+      apply in_or_app. right. simpl. auto.
+    eapply wf_system__wf_cmd with (c:=c') in Hwfc; eauto.
+    split.
+    SSCase "1.1".
+      destruct cs'; simpl_env in *.
+      SSSCase "1.1.1".
+        assert (~ In (getCmdLoc c') (getCmdsLocs cs2')) as Hnotin.
+          eapply wf_system__uniq_block with (f:=F') in HwfSystem; eauto.        
+          simpl in HwfSystem.
+          apply NoDup_inv in HwfSystem.
+          destruct HwfSystem as [_ J].
+          apply NoDup_inv in J.
+          destruct J as [J _].
+          rewrite getCmdsLocs_app in J.
+          simpl in J.
+          apply NoDup_last_inv in J. auto.
+        apply inscope_of_cmd_tmn in HeqR2; auto.
+        destruct HeqR2 as [ids2 [J1 J2]].        
+        rewrite <- J1.
+        remember (getCmdID c') as R.
+        destruct c'; try solve [inversion H].
+        unfold SBopsem.returnUpdateLocals in H1. simpl in H1.
+        destruct R.
+          destruct n; inv HeqR.
+          remember (getOperandValue (los,nts) Mem' Result lc gl) as R1.
+          destruct R1; inv H1.          
+          inv Hwfc. 
+          remember (SBopsem.get_reg_metadata (los, nts) Mem' gl rm Result) 
+            as R2.
+          unfold SBopsem.prop_reg_metadata in H3.
+          assert (wf_defs F' (updateAddAL GenericValue lc' i0 g) ids2) as J.
+            eapply wf_defs_updateAddAL with (t1:=typ1) ; eauto.
+              eapply uniqF__lookupTypViaIDFromFdef; eauto.
+                eapply wf_system__uniqFdef; eauto.
+          destruct typ1; inv H3; auto.
+            destruct (get_reg_metadata (los, nts) Mem' gl rm Result) as 
+              [[md ?]|]; inv H2; auto.
+
+          destruct n; inv HeqR. inv H1.
+          eapply wf_defs_eq; eauto. 
+        
+      SSSCase "1.1.2".
+        assert (NoDup (getCmdsLocs (cs2' ++ [c'] ++ [c] ++ cs'))) as Hnodup.
+          eapply wf_system__uniq_block with (f:=F') in HwfSystem; eauto.        
+          simpl in HwfSystem.
+          apply NoDup_inv in HwfSystem.
+          destruct HwfSystem as [_ J].
+          apply NoDup_inv in J.
+          destruct J as [J _]. auto.
+        apply inscope_of_cmd_cmd in HeqR2; auto.
+        destruct HeqR2 as [ids2 [J1 J2]].        
+        rewrite <- J1.
+        remember (getCmdID c') as R.
+        destruct c'; try solve [inversion H].
+        unfold SBopsem.returnUpdateLocals in H1. simpl in H1.
+        destruct R.
+          destruct n; inv HeqR.
+          remember (getOperandValue (los,nts) Mem' Result lc gl) as R1.
+          destruct R1; inv H1.
+          inv Hwfc.
+          remember (SBopsem.get_reg_metadata (los, nts) Mem' gl rm Result) 
+            as R2.
+          unfold SBopsem.prop_reg_metadata in H3.
+          assert (wf_defs F' (updateAddAL GenericValue lc' i0 g) ids2) as J.
+            eapply wf_defs_updateAddAL with (t1:=typ1) ; eauto.
+              eapply uniqF__lookupTypViaIDFromFdef; eauto.
+                eapply wf_system__uniqFdef; eauto.
+          destruct typ1; inv H3; auto.
+            destruct (get_reg_metadata (los, nts) Mem' gl rm Result) as 
+              [[md ?]|]; inv H2; auto.
+
+          destruct n; inv HeqR. inv H1.
+          eapply wf_defs_eq; eauto. 
+
+    split.
+    SSCase "1.2".
+      clear HeqR2 HwfCall HwfCall' HinCs Hreach2 HwfEC H0 Hwfg H Hreach1 HBinF1.
+      clear HeqR1 Hinscope1 Hinscope2 HFinPs1 Hwfm1.
+      eapply returnUpdateLocals__wf_rmap; eauto.
+
+    SSCase "1.3".
+      exists l2. exists ps2. exists (cs2'++[c']).   
+      simpl_env. auto.
+Unfocus.
+
+Focus.
+Case "dsReturnVoid".
+  destruct HwfS1 as 
+    [Hwfg [HwfSystem [HmInS [
+     [Hreach1 [HBinF1 [HFinPs1 [Hinscope1 [Hwfm1 [l1 [ps1 [cs1' Heq1]]]]]]]]
+     [
+       [
+         [Hreach2 [HBinF2 [HFinPs2 [Hinscope2 [Hwfm2 [l2 [ps2 [cs2' Heq2]]]]]]]]
+         [HwfEC HwfCall]
+       ]
+       HwfCall'
+     ]
+    ]]]]; subst.
+  remember (inscope_of_cmd F' (block_intro l2 ps2 (cs2' ++ c' :: cs') tmn') c')
+    as R2.
+  destruct R2; try solve [inversion Hinscope2].
+  remember (inscope_of_tmn F
+             (block_intro l1 ps1 (cs1' ++ nil)(insn_return_void rid))
+             (insn_return_void rid)) as R1. 
+  destruct R1; try solve [inversion Hinscope1].
+  split; auto.
+  split; auto.
+  SCase "1".
+    split; auto.
+    split; auto.
+    split; auto.
+    split; auto.
+    split; auto.
+    split.   
+    SSCase "1.1".
+      apply HwfCall' in HBinF1. simpl in HBinF1.
+      destruct cs'; simpl_env in *.
+      SSSCase "1.1.1".
+        assert (~ In (getCmdLoc c') (getCmdsLocs cs2')) as Hnotin.
+          eapply wf_system__uniq_block with (f:=F') in HwfSystem; eauto.        
+          simpl in HwfSystem.
+          apply NoDup_inv in HwfSystem.
+          destruct HwfSystem as [_ J].
+          apply NoDup_inv in J.
+          destruct J as [J _].
+          rewrite getCmdsLocs_app in J.
+          simpl in J.
+          apply NoDup_last_inv in J. auto.
+        clear - HeqR2 Hinscope2 H HwfCall' HBinF1 Hnotin H1.
+        apply inscope_of_cmd_tmn in HeqR2; auto.
+        destruct HeqR2 as [ids2 [J1 J2]].        
+        rewrite <- J1.
+        remember (getCmdID c') as R.
+        destruct c'; try solve [inversion H].
+        destruct n; inversion H1.
+        simpl in HeqR. subst R.
+        eapply wf_defs_eq; eauto. 
+        
+      SSSCase "1.1.2".
+        assert (NoDup (getCmdsLocs (cs2' ++ [c'] ++ [c] ++ cs'))) as Hnodup.
+          eapply wf_system__uniq_block with (f:=F') in HwfSystem; eauto.        
+          simpl in HwfSystem.
+          apply NoDup_inv in HwfSystem.
+          destruct HwfSystem as [_ J].
+          apply NoDup_inv in J.
+          destruct J as [J _]. auto.
+        clear - HeqR2 Hinscope2 H HwfCall' HBinF1 Hnodup H1.
+        apply inscope_of_cmd_cmd in HeqR2; auto.
+        destruct HeqR2 as [ids2 [J1 J2]].        
+        rewrite <- J1.
+        remember (getCmdID c') as R.
+        destruct c'; try solve [inversion H].
+        destruct n; inversion H1.
+        simpl in HeqR. subst R.
+        eapply wf_defs_eq; eauto. 
+
+    split; auto.
+    SSCase "1.3".
+      exists l2. exists ps2. exists (cs2'++[c']).   
+      simpl_env. auto.
+Unfocus.
+
+Focus.
+Case "dsBranch".
+  destruct HwfS1 as 
+    [Hwfg [HwfSystem [HmInS [
+     [Hreach1 [HBinF1 [HFinPs1 [Hinscope1 [Hwfm1 [l3 [ps3 [cs3' Heq1]]]]]]]]
+     [HwfEC HwfCall]]]]
+    ]; subst.
+  remember (inscope_of_tmn F
+             (block_intro l3 ps3 (cs3' ++ nil)(insn_br bid Cond l1 l2))
+             (insn_br bid Cond l1 l2)) as R1. 
+  destruct R1; try solve [inversion Hinscope1].
+  split; auto.
+  split; auto.
+  split; auto.
+  split; auto.
+    assert (uniqFdef F) as HuniqF.
+      eapply wf_system__uniqFdef in HwfSystem; eauto.   
+    assert (blockInFdefB (block_intro l' ps' cs' tmn') F = true) as HBinF.
+      clear - H0 HBinF1 HFinPs1 HmInS HwfSystem HuniqF.
+      destruct (isGVZero (los, nts) c).
+        symmetry in H0.
+        apply lookupBlockViaLabelFromFdef_inv in H0; auto.
+          destruct H0; auto.
+        symmetry in H0.
+        apply lookupBlockViaLabelFromFdef_inv in H0; auto.
+          destruct H0; auto.
+    split.
+      clear - Hreach1 H0 HBinF1 HFinPs1 HmInS HwfSystem HuniqF.
+      unfold isReachableFromEntry in *.
+      destruct (isGVZero (los, nts) c).
+        symmetry in H0.
+        apply lookupBlockViaLabelFromFdef_inv in H0; eauto.
+        destruct H0 as [H0 _].
+        eapply reachable_successors; eauto.
+          simpl. auto.
+      
+        symmetry in H0.
+        apply lookupBlockViaLabelFromFdef_inv in H0; eauto.
+        destruct H0 as [H0 _].
+        eapply reachable_successors; eauto.
+          simpl. auto.
+    split; auto.
+    split; auto.
+    split.
+      assert (HwfF := HwfSystem).
+      eapply wf_system__wf_fdef with (f:=F) in HwfF; eauto.
+      clear - H0 HeqR1 H1 Hinscope1 H HwfSystem HBinF1 HwfF HuniqF.
+      eapply inscope_of_tmn_br in HeqR1; eauto.
+        destruct HeqR1 as [ids0' [HeqR1 [J1 J2]]].
+        destruct cs'; rewrite <- HeqR1; eauto.
+
+        eapply switchToNewBasicBlock_sim; eauto.
+
+    split.
+      clear HwfEC Hreach1 HwfCall Hwfg HeqR1 Hinscope1 H.
+      eapply switchToNewBasicBlock__wf_rmap with 
+        (b1:=block_intro l' ps' cs' tmn')
+        (b2:=block_intro l3 ps3 (cs3' ++ nil) (insn_br bid Cond l1 l2)); eauto.
+
+      exists l'. exists ps'. exists nil. simpl_env. auto.
+Unfocus.
+
+Focus.
+Case "dsBranch_uncond".
+  destruct HwfS1 as 
+    [Hwfg [HwfSystem [HmInS [
+     [Hreach1 [HBinF1 [HFinPs1 [Hinscope1 [Hwfm1 [l3 [ps3 [cs3' Heq1]]]]]]]] 
+     [HwfEC HwfCall]]]]
+    ]; subst.
+  remember (inscope_of_tmn F
+             (block_intro l3 ps3 (cs3' ++ nil)(insn_br_uncond bid l0))
+             (insn_br_uncond bid l0)) as R1. 
+  destruct R1; try solve [inversion Hinscope1].
+  split; auto.
+  split; auto.
+  split; auto.
+  SCase "1".
+    assert (uniqFdef F) as HuniqF.
+      eapply wf_system__uniqFdef in HwfSystem; eauto.   
+    assert (H':=H).
+    symmetry in H'.
+    apply lookupBlockViaLabelFromFdef_inv in H'; auto.
+    destruct H' as [EQ HBinF]; subst.
+    split; auto.
+    split.
+      clear - Hreach1 HBinF1 HFinPs1 HmInS HwfSystem HuniqF HBinF.
+      unfold isReachableFromEntry in *.
+      eapply reachable_successors; eauto.
+        simpl. auto.
+    split; auto.
+    split; auto.
+    split.
+      assert (HwfF := HwfSystem).
+      eapply wf_system__wf_fdef with (f:=F) in HwfF; eauto.
+      clear - H0 HeqR1 Hinscope1 HwfSystem HBinF1 HwfF HuniqF HBinF H.
+      assert (Hwds := HeqR1).
+      eapply inscope_of_tmn_br_uncond with (cs':=cs')(l':=l')(ps':=ps')
+        (tmn':=tmn') in HeqR1; eauto.
+        destruct HeqR1 as [ids0' [HeqR1 [J1 J2]]].
+        destruct cs'; rewrite <- HeqR1; eauto.
+
+        eapply switchToNewBasicBlock_sim; eauto.
+
+    split.
+      clear HwfEC Hreach1 HwfCall Hwfg HeqR1 Hinscope1.
+      eapply switchToNewBasicBlock__wf_rmap 
+        with (b1:=block_intro l' ps' cs' tmn'); eauto.
+
+      exists l'. exists ps'. exists nil. simpl_env. auto.
+Unfocus.
+
+Case "dsBop". preservation_tac HwfS1.
+Case "dsFBop". preservation_tac HwfS1. 
+Case "dsExtractValue".
+  assert (exists t0, getSubTypFromConstIdxs idxs t = Some t0) as J.
+    destruct HwfS1 as 
+      [Hwfg [HwfSystem [HmInS [
+         [Hreach1 [HBinF1 [HFinPs1 [Hinscope1 [Hwfm1 [l3 [ps3 [cs3' Heq1]]]]]]]] 
+         [HwfEC HwfCall]]]]
+      ]; subst.
+    eapply wf_system__wf_cmd with (c:=insn_extractvalue id0 t v idxs) in HBinF1; 
+      eauto.
+      inv HBinF1; eauto.
+      apply in_or_app; simpl; auto.
+
+  destruct J as [t0 J].
+  eapply preservation_cmd_updated_case in HwfS1; simpl; eauto.
+    intro J0. 
+    apply updateAddAL_nptr__wf_rmap; auto.
+      apply wf_State__cmd__lookupTypViaIDFromFdef in HwfS1.
+      rewrite HwfS1; simpl; auto. 
+        rewrite J. 
+          admit. (* unsupported *)
+Case "dsInsertValue". 
+  eapply preservation_cmd_updated_case with (rm':=rm) in HwfS1; simpl; eauto.
+    intro J. 
+    apply updateAddAL_nptr__wf_rmap; auto.
+      apply wf_State__cmd__lookupTypViaIDFromFdef in HwfS1.
+      rewrite HwfS1; simpl; auto. 
+        admit. (* unsupported *)
+Case "dsMalloc". 
+  eapply preservation_cmd_updated_case with (rm':=
+          updateAddAL SBopsem.metadata rm id0
+            {| SBopsem.md_base := SBopsem.base2GV (los, nts) mb;
+               SBopsem.md_bound := SBopsem.bound2GV (los, nts) mb tsz n |})
+   in HwfS1; simpl; eauto.
+    apply updateAddAL_ptr__wf_rmap; auto. 
+Case "dsFree". 
+  eapply preservation_cmd_non_updated_case with (MM':=MM) in HwfS1; eauto.
+Case "dsAlloca".
+  eapply preservation_cmd_updated_case with (rm':=
+          updateAddAL SBopsem.metadata rm id0
+            {| SBopsem.md_base := SBopsem.base2GV (los, nts) mb;
+               SBopsem.md_bound := SBopsem.bound2GV (los, nts) mb tsz n |})
+   in HwfS1; simpl; eauto.
+    apply updateAddAL_ptr__wf_rmap; auto. 
+Case "dsLoad_nptr". 
+  eapply preservation_cmd_updated_case with (rm':=rm) in HwfS1; simpl; eauto.
+    intro J0. 
+    apply updateAddAL_nptr__wf_rmap; auto.
+      apply wf_State__cmd__lookupTypViaIDFromFdef in HwfS1.
+      rewrite HwfS1; simpl; auto. 
+        intros t0 EQ. inv EQ. inv H3.
+Case "dsLoad_ptr".
+  eapply preservation_cmd_updated_case with (rm':=updateAddAL metadata rm id0
+    (get_mem_metadata (los, nts) MM gvp)) in HwfS1; simpl; eauto.
+    apply updateAddAL_ptr__wf_rmap; auto. 
+Case "dsStore_nptr". 
+  eapply preservation_cmd_non_updated_case with (MM':=MM) in HwfS1; eauto.
+Case "dsStore_ptr". 
+  eapply preservation_cmd_non_updated_case with (MM':=MM') in HwfS1; eauto.
+Case "dsGEP". 
+  assert (exists t0, getGEPTyp idxs t = Some t0) as J.
+    destruct HwfS1 as 
+      [Hwfg [HwfSystem [HmInS [
+         [Hreach1 [HBinF1 [HFinPs1 [Hinscope1 [Hwfm1 [l3 [ps3 [cs3' Heq1]]]]]]]] 
+         [HwfEC HwfCall]]]]
+      ]; subst.
+    eapply wf_system__wf_cmd with(c:=insn_gep id0 inbounds0 t vp idxs) in HBinF1;
+      eauto.
+      inv HBinF1; eauto.
+      apply in_or_app; simpl; auto.
+  destruct J as [t0 J].
+  eapply preservation_cmd_updated_case with 
+    (rm':=updateAddAL SBopsem.metadata rm id0 md) in HwfS1; simpl; eauto.
+    apply updateAddAL_ptr__wf_rmap; auto.
+Case "dsTrunc".
+  eapply preservation_cmd_updated_case with (rm':=rm) in HwfS1; simpl; eauto.
+    intro J0. 
+    apply updateAddAL_nptr__wf_rmap; auto.
+      assert (Htyp:=HwfS1).
+      apply wf_State__cmd__lookupTypViaIDFromFdef in Htyp.
+      rewrite Htyp; simpl; auto. 
+        apply wf_State__wf_cmd in HwfS1.
+        inv HwfS1. inv H6; congruence.
+Case "dsExt". 
+  eapply preservation_cmd_updated_case with (rm':=rm) in HwfS1; simpl; eauto.
+    intro J0. 
+    apply updateAddAL_nptr__wf_rmap; auto.
+      assert (Htyp:=HwfS1).
+      apply wf_State__cmd__lookupTypViaIDFromFdef in Htyp.
+      rewrite Htyp; simpl; auto. 
+        apply wf_State__wf_cmd in HwfS1.
+        inv HwfS1. inv H6; congruence.
+Case "dsBitcast_nptr". 
+  eapply preservation_cmd_updated_case with (rm':=rm) in HwfS1; simpl; eauto.
+    intro J0. 
+    apply updateAddAL_nptr__wf_rmap; auto.
+      assert (Htyp:=HwfS1).
+      apply wf_State__cmd__lookupTypViaIDFromFdef in Htyp.
+      rewrite Htyp; simpl; auto. 
+        apply wf_State__wf_cmd in HwfS1.
+        inv HwfS1. inv H7; try congruence.
+          inv H0.
+Case "dsBitcast_ptr". 
+  eapply preservation_cmd_updated_case with (rm':=updateAddAL metadata rm id0 md)
+    in HwfS1; simpl; eauto.
+    apply updateAddAL_ptr__wf_rmap; auto.
+Case "dsInttoptr". 
+  eapply preservation_cmd_updated_case with (rm':=
+    updateAddAL SBopsem.metadata rm id0 
+      {| SBopsem.md_base := null;
+         SBopsem.md_bound := null |}) in HwfS1; simpl; eauto.
+    apply updateAddAL_ptr__wf_rmap; auto.
+Case "dsOthercast". 
+  eapply preservation_cmd_updated_case with (rm':=rm) in HwfS1; simpl; eauto.
+    intro J0. 
+    apply updateAddAL_nptr__wf_rmap; auto.
+      assert (Htyp:=HwfS1).
+      apply wf_State__cmd__lookupTypViaIDFromFdef in Htyp.
+      rewrite Htyp; simpl; auto. 
+        apply wf_State__wf_cmd in HwfS1.
+        inv HwfS1. 
+        destruct H0 as [J1 J2]. 
+        inv H7; try (congruence).
+Case "dsIcmp". 
+  eapply preservation_cmd_updated_case with (rm':=rm) in HwfS1; simpl; eauto.
+    intro J0. 
+    apply updateAddAL_nptr__wf_rmap; auto.
+      assert (Htyp:=HwfS1).
+      apply wf_State__cmd__lookupTypViaIDFromFdef in Htyp.
+      rewrite Htyp; simpl; auto. 
+        apply wf_State__wf_cmd in HwfS1.
+        inv HwfS1. congruence.
+Case "dsFcmp". 
+  eapply preservation_cmd_updated_case with (rm':=rm) in HwfS1; simpl; eauto.
+    intro J0. 
+    apply updateAddAL_nptr__wf_rmap; auto.
+      assert (Htyp:=HwfS1).
+      apply wf_State__cmd__lookupTypViaIDFromFdef in Htyp.
+      rewrite Htyp; simpl; auto. 
+        apply wf_State__wf_cmd in HwfS1.
+        inv HwfS1. congruence.
+Case "dsSelect_nptr".
+  destruct (isGVZero (los, nts) c); 
+  eapply preservation_cmd_updated_case with (rm':=rm) in HwfS1; simpl; 
+    try solve [
+      eauto |
+      intro J0;
+      apply updateAddAL_nptr__wf_rmap; try solve [
+        auto |
+        apply wf_State__cmd__lookupTypViaIDFromFdef in HwfS1;
+          rewrite HwfS1; simpl; try solve [auto | intros t0 EQ; inv EQ; inv H2]
+      ]
+    ].
+
+Case "dsSelect_ptr".
+  destruct (isGVZero (los, nts) c); try invert_prop_reg_metadata.
+    eapply preservation_cmd_updated_case with 
+      (rm':=updateAddAL metadata rm id0 md2) in HwfS1; simpl; 
+      try solve [eauto | apply updateAddAL_ptr__wf_rmap; auto].
+    eapply preservation_cmd_updated_case with 
+      (rm':=updateAddAL metadata rm id0 md1) in HwfS1; simpl; 
+      try solve [eauto | apply updateAddAL_ptr__wf_rmap; auto].
+
+Focus.
+Case "dsCall".
+  destruct HwfS1 as [Hwfg [HwfSys [HmInS [HwfEC [HwfECs HwfCall]]]]].
+  assert (InProductsB (product_fdef (fdef_intro 
+    (fheader_intro fa rt fid la va) lb)) Ps = true) as HFinPs'.
+    eapply lookupFdefViaGV_inv; eauto.
+  split; auto.
+  split; auto.
+  split; auto.
+  split.
+  SCase "1".     
+    split.
+      simpl. eapply reachable_entrypoint; eauto.
+    split.
+     apply entryBlockInFdef in H0; auto.
+    split; auto.
+    split.
+     assert (ps'=nil) as EQ.
+       eapply entryBlock_has_no_phinodes with (ifs:=nil)(s:=S); eauto.        
+     subst.
+     apply dom_entrypoint in H0.
+     eapply initLocals_params2GVs_sim in H1; eauto.
+      destruct H1 as [gvs [J1 J2]]; subst.
+     destruct cs'.
+       unfold inscope_of_tmn.
+       remember ((dom_analyze (fdef_intro (fheader_intro fa rt fid la va) lb)) 
+         !! l') as R.
+       destruct R.
+       destruct HwfEC as [Hreach [HBinF [HFinPs [Hinscope [l1 [ps [cs' Heq]]]]]]]
+         ; subst.       
+       eapply preservation_dbCall_case; eauto.
+
+       unfold inscope_of_cmd.
+       remember ((dom_analyze (fdef_intro (fheader_intro fa rt fid la va) lb)) 
+         !! l') as R.
+       destruct R. simpl.
+       destruct (eq_atom_dec (getCmdLoc c) (getCmdLoc c)) as [|n]; 
+         try solve [contradict n; auto]. 
+       eapply preservation_dbCall_case; eauto.
+    split.
+      eapply initLocals__wf_rmap; eauto.
+
+      exists l'. exists ps'. exists nil. simpl_env. auto.
+  split.
+  SCase "2".
+    split; auto.
+  SCase "3".
+    simpl. intros b HbInBs. destruct b.
+    destruct t; auto.
+
+Unfocus.
+
+Case "dsExCall". 
+  unfold exCallUpdateLocals in H2.
+  destruct noret0.
+    inv H2.
+    eapply preservation_cmd_non_updated_case with (MM':=MM) in HwfS1; eauto.
+
+    destruct oresult; inv H2.
+    assert (exists t0, getCmdTyp (insn_call rid false ca ft fv lp) = Some t0)
+      as J.
+      destruct HwfS1 as 
+        [Hwfg [HwfSystem [HmInS [
+         [Hreach1 [HBinF1 [HFinPs1 [Hinscope1 [Hwfm1 [l3 [ps3 [cs3' Heq1]]]]]]]] 
+         [HwfEC HwfCall]]]]
+        ]; subst.
+      eapply wf_system__wf_cmd with (c:=insn_call rid false ca ft fv lp) 
+        in HBinF1; eauto.
+      simpl.
+      inv HBinF1; eauto. 
+      apply in_or_app; simpl; auto.
+
+    destruct J as [t0 J].
+    destruct ft; inv H4; try solve [
+      eapply preservation_cmd_updated_case with (t0:=t0)(rm':=rm') in HwfS1; 
+        try solve [eauto |
+          intro J0;
+          apply updateAddAL_nptr__wf_rmap; try solve [auto |
+            apply wf_State__cmd__lookupTypViaIDFromFdef in HwfS1;
+            rewrite HwfS1; simpl; try solve [auto | congruence]]
+        ]
+    ].    
+    destruct ft; inv H3; try solve [
+      eapply preservation_cmd_updated_case with (t0:=t0)
+        (rm':=updateAddAL metadata rm rid
+          {| md_base := gundef; md_bound := gundef |}) in HwfS1; 
+        try solve [eauto | intro J0; apply updateAddAL_ptr__wf_rmap; auto] |
+      eapply preservation_cmd_updated_case with (t0:=t0)(rm':=rm') in HwfS1; 
+        try solve [eauto |
+          intro J0;
+          apply updateAddAL_nptr__wf_rmap; try solve [auto |
+            apply wf_State__cmd__lookupTypViaIDFromFdef in HwfS1;
+            rewrite HwfS1; simpl; try solve [auto | congruence]]
+        ]
+    ].
+Qed.
+
+(*********************************************)
+(** * Progress *)
+
+Definition memory_violation S : Prop :=
+  match S with
+  | {| SBopsem.CurTargetData := TD;
+       SBopsem.ECS := {| SBopsem.CurCmds := insn_load _ t vp _ :: cs;
+                           SBopsem.Locals := lc;
+                           SBopsem.Rmap := rm
+                         |} :: _;
+        SBopsem.Globals := gl;
+        SBopsem.Mem := Mem0 |} => 
+      match SBopsem.get_reg_metadata TD Mem0 gl rm vp, 
+            getOperandValue TD Mem0 vp lc gl with
+      | ret (md, mt), ret gvp => ~ SBopsem.assert_mptr TD t gvp md
+      | _, _ => False
+      end
+  | {| SBopsem.CurTargetData := TD;
+       SBopsem.ECS := {| SBopsem.CurCmds := insn_store _ t v vp _ :: cs;
+                           SBopsem.Locals := lc;
+                           SBopsem.Rmap := rm
+                         |} :: _;
+        SBopsem.Globals := gl;
+        SBopsem.Mem := Mem0 |} => 
+      match SBopsem.get_reg_metadata TD Mem0 gl rm vp, 
+            getOperandValue TD Mem0 vp lc gl with
+      | ret (md, mt), ret gvp => ~ SBopsem.assert_mptr TD t gvp md
+      | _, _ => False
+      end
+  | _ => False
+  end.
+
+Definition undefined_state S : Prop :=
+  match S with
+  | {| SBopsem.CurTargetData := td;
+       SBopsem.ECS := {|
+                SBopsem.CurCmds := nil;
+                SBopsem.Terminator := insn_return _ _ _;
+                SBopsem.Allocas := als |} :: 
+              {| SBopsem.CurCmds := c::_ |} :: _;
+       SBopsem.Mem := M |} => free_allocas td M als = None
+  | _ => False
+  end \/
+  match S with
+  | {| SBopsem.CurTargetData := td;
+       SBopsem.ECS := {|
+                SBopsem.CurBB := _;
+                SBopsem.CurCmds := nil;
+                SBopsem.Terminator := insn_return_void _;
+                SBopsem.Allocas := als |} :: 
+              {| SBopsem.CurCmds := c::_ |} :: _;
+       SBopsem.Mem := M |} => 
+                      free_allocas td M als = None \/ 
+                      match getCallerReturnID c with
+                      | Some _ => True
+                      | _ => False
+                      end
+  | _ => False
+  end \/
+  match S with
+  | {| SBopsem.ECS := {|
+                SBopsem.CurBB := block_intro _ _ _ (insn_unreachable _);
+                SBopsem.CurCmds := nil;
+                SBopsem.Terminator := (insn_unreachable _)
+               |} :: _
+     |} => True
+  | _ => False
+  end \/
+  match S with
+  | {| SBopsem.CurTargetData := td;
+       SBopsem.ECS := 
+         {| SBopsem.CurCmds := insn_malloc _ t v a::_ ; 
+            SBopsem.Locals := lc|} :: _;
+       SBopsem.Globals := gl;
+      SBopsem.Mem := M |}
+  | {| SBopsem.CurTargetData := td;
+       SBopsem.ECS := 
+         {| SBopsem.CurCmds := insn_alloca _ t v a::_ ; 
+            SBopsem.Locals := lc|} :: _;
+       SBopsem.Globals := gl;
+       SBopsem.Mem := M |} =>
+       match getOperandValue td M v lc gl with
+       | Some gv =>
+           match getTypeAllocSize td t with
+           | Some asz =>
+               match malloc td M asz gv a with
+               | None => True
+               | _ => False
+               end
+           | _ => False
+           end
+       | _ => False
+       end
+  | _ => False
+  end \/
+  match S with
+  | {| SBopsem.CurTargetData := td;
+       SBopsem.ECS := 
+         {| SBopsem.CurCmds := insn_free _ _ v::_ ; SBopsem.Locals := lc|} 
+         :: _;
+       SBopsem.Globals := gl;
+       SBopsem.Mem := M |} =>
+       match getOperandValue td M v lc gl with
+       | Some gv =>
+           match free td M gv with
+           | None => True
+           | _ => False
+           end
+       | _ => False
+       end
+  | _ => False
+  end \/
+  match S with
+  | {| SBopsem.CurTargetData := td;
+       SBopsem.ECS := 
+         {| SBopsem.CurCmds := insn_load _ t v a::_ ; 
+            SBopsem.Locals := lc|} :: _;
+       SBopsem.Globals := gl;
+       SBopsem.Mem := M |} =>
+       match getOperandValue td M v lc gl with
+       | Some gv =>
+           match mload td M gv t a with
+           | None => True
+           | _ => False
+           end
+       | _ => False
+       end
+  | _ => False
+  end \/
+  match S with
+  | {| SBopsem.CurTargetData := td;
+       SBopsem.ECS := 
+         {| SBopsem.CurCmds := insn_store _ t v v0 a::_ ; 
+            SBopsem.Locals := lc|} :: _;
+       SBopsem.Globals := gl;
+       SBopsem.Mem := M |} =>
+       match getOperandValue td M v lc gl, getOperandValue td M v0 lc gl with
+       | Some gv, Some mgv =>
+           match mstore td M mgv t gv a with
+           | None => True
+           | _ => False
+           end
+       | _, _ => False
+       end
+  | _ => False
+  end \/
+  match S with
+  | {| SBopsem.CurTargetData := td;
+       SBopsem.CurProducts := ps;
+       SBopsem.ECS := 
+         {| SBopsem.CurCmds := insn_call i0 n _ ft v p::_ ; 
+            SBopsem.Locals := lc; SBopsem.Rmap := rm |} :: _;
+       SBopsem.Globals := gl;
+       SBopsem.FunTable := fs;
+       SBopsem.Mem := M |} =>
+       match lookupFdefViaGV td M ps gl lc fs v, 
+             lookupExFdecViaGV td M ps gl lc fs v with
+       | None, Some (fdec_intro (fheader_intro fa rt fid la va)) =>
+           match LLVMgv.params2GVs td M p lc gl with
+           | Some gvs =>
+             match LLVMopsem.callExternalFunction M fid gvs with
+             | (oresult, _) =>
+                match exCallUpdateLocals ft n i0 oresult lc rm with
+                | None => True
+                | _ => False
+                end
+             end
+           | _ => False
+           end
+       | None, None => True
+       | _, _ => False
+       end
+  | _ => False
+  end \/
+  memory_violation S.
+
+Ltac undefbehave := unfold undefined_state; simpl; 
+  try solve [
+    auto | 
+    right; auto | 
+    right; right; auto |  
+    right; right; right; right; auto |
+    right; right; right; right; right; auto |
+    right; right; right; right; right; right; auto |
+    right; right; right; right; right; right; right; auto |
+    right; right; right; right; right; right; right; right; auto
+  ].
+
+Hint Constructors SBopsem.dsInsn.
+
+Lemma assert_mptr_dec : forall TD t ptr md,
+  SBopsem.assert_mptr TD t ptr md \/ ~ SBopsem.assert_mptr TD t ptr md.
+Proof.
+  intros.
+  unfold is_true. 
+  destruct (SBopsem.assert_mptr TD t ptr md); auto.
+Qed.
+
+Lemma get_const_metadata_isnt_stuck : forall TD M gl vc gv bc ec t1,
+  const2GV TD M gl vc = Some gv ->
+  get_const_metadata vc = Some (bc, ec, t1) ->
+  exists gvb, exists gve, 
+    const2GV TD M gl bc = Some gvb /\ const2GV TD M gl ec = Some gve.
+Proof.
+  unfold const2GV.
+  intros TD M gl vc gv bc ec t1 J1 J2.  
+  remember (_const2GV TD M gl vc) as J3.
+  destruct J3 as [[gv3 t3]|]; inv J1.
+  generalize dependent gv.
+  generalize dependent t3.
+  generalize dependent ec.
+  generalize dependent bc.
+  generalize dependent t1.
+  induction vc; intros; try solve [inversion J2].
+    exists gv.
+    remember t as T.
+    destruct T; inversion J2; clear J2; subst bc ec t1; simpl in *; try solve [
+      destruct (lookupAL GenericValue gl i0); inversion HeqJ3; subst gv t3;
+      destruct (GV2ptr TD (getPointerSize TD) g); eauto;
+      remember (mgep TD t v 
+        (INTEGER.to_Z (INTEGER.of_Z 32 1 false) :: nil)) as optr;
+      subst t; rewrite <- Heqoptr;
+      destruct optr; eauto
+    ].
+
+    simpl in *.
+    remember (_const2GV TD M gl vc) as R.
+    destruct R as [[gv2 t2]|]; try solve [inv HeqJ3].
+    apply IHvc with (gv:=gv2)(t3:=t2) in J2; auto.
+Qed.
+
+Lemma wf_phinodes__getIncomingValuesForBlockFromPHINodes : forall
+  (s : system)
+  (los : layouts)
+  (nts : namedts)
+  (ps : list product)
+  (f : fdef)
+  l0
+  (lc : GVMap)
+  (gl : GVMap)
+  (M : mem)
+  (t : list atom)
+  l1 ps1 cs1 tmn1
+  (Hwfg : wf_global s gl)
+  (HeqR : ret t = inscope_of_tmn f (block_intro l1 ps1 cs1 tmn1) tmn1)
+  (Hinscope : wf_defs f lc t)
+  (HuniqF : uniqFdef f)
+  (ps' : phinodes)
+  (cs' : cmds)
+  (tmn' : terminator)
+  ps2
+  (Hreach : isReachableFromEntry f (block_intro l0 ps' cs' tmn'))
+  (HbInF : blockInFdefB
+            (block_intro l1 ps1 cs1 tmn1) f = true)
+  (HwfB : wf_block nil s (module_intro los nts ps) f 
+             (block_intro l1 ps1 cs1 tmn1))
+  (H8 : wf_phinodes nil s (module_intro los nts ps) f
+         (block_intro l0 ps' cs' tmn') ps2)
+  (Hsucc : In l0 (successors_terminator tmn1))
+  rm (Hwfm: wf_rmap f lc rm)
+  (Hin: exists ps1, ps' = ps1 ++ ps2),
+   exists RVs : list (id * GenericValue * option (metadata * typ)),
+     getIncomingValuesForBlockFromPHINodes (los, nts) M ps2 
+       (block_intro l1 ps1 cs1 tmn1) gl lc rm =
+       ret RVs.
+Proof.
+  intros.
+  induction ps2; simpl.
+    exists nil. auto.
+  
+    destruct a. inv H8. inv H6.
+    assert (exists v, getValueViaLabelFromValuels l2 l1 = Some v) as J.      
+      clear - H14 HbInF HuniqF Hsucc.
+      inv H14.
+      unfold check_list_value_l in H0.
+      remember (split (unmake_list_value_l l2)) as R.
+      destruct R.
+      destruct H0 as [J1 [J2 J3]].
+      eapply In__getValueViaLabelFromValuels; eauto.
+      destruct J2 as [_ J2].
+      apply J2.
+      eapply successors_predOfBlock; eauto.
+
+    destruct J as [v J].
+    rewrite J.
+    assert (HwfV:=J).
+    eapply wf_value_list__getValueViaLabelFromValuels__wf_value in HwfV; eauto.
+    destruct v as [vid | vc].
+    Case "vid".
+      assert (exists gv1, lookupAL GenericValue lc vid = Some gv1) as J1.
+        Focus.
+        destruct H14 as [Hwfops Hwfvls].             
+        assert (Hnth:=J).
+        eapply getValueViaLabelFromValuels__nth_list_value_l in Hnth; eauto.
+        destruct Hnth as [n Hnth].
+        eapply wf_phi_operands__elim in Hwfops; eauto.
+        destruct Hwfops as [Hneqid [vb [b1 [Hlkvb [Hlkb1 Hdom]]]]].
+        assert (b1 = block_intro l1 ps1 cs1 tmn1) 
+          as EQ.
+          clear - Hlkb1 HbInF HuniqF.
+          apply blockInFdefB_lookupBlockViaLabelFromFdef in HbInF; auto.
+          rewrite HbInF in Hlkb1. inv Hlkb1; auto.
+
+        subst.
+        clear - Hdom Hinscope HeqR J Hreach H2 HbInF Hlkvb Hlkb1 HuniqF.
+        destruct Hdom as [J3 | J3]; try solve [contradict Hreach; auto].
+        clear Hreach.        
+        unfold blockDominates in J3.         
+        destruct vb.
+        unfold inscope_of_tmn in HeqR.
+        destruct f. destruct f.
+        remember ((dom_analyze (fdef_intro (fheader_intro f t2 i0 a v) b)) !! l1)
+          as R1.
+        destruct R1.
+        symmetry in HeqR.    
+        apply fold_left__spec in HeqR.
+        destruct (eq_atom_dec l3 l1); subst.
+        SCase "l3=l1".
+          destruct HeqR as [HeqR _].
+          assert (In vid t) as G.
+            clear - J HeqR Hlkb1 J3 Hlkvb HbInF HuniqF.
+            assert (J':=Hlkvb).
+            apply lookupBlockViaIDFromFdef__blockInFdefB in Hlkvb.
+            apply lookupBlockViaLabelFromFdef_inv in Hlkb1; auto.
+            destruct Hlkb1 as [J1 J2].
+            eapply blockInFdefB_uniq in J2; eauto.
+            destruct J2 as [J2 [J4 J5]]; subst.
+            apply lookupBlockViaIDFromFdef__InGetBlockIDs in J'.
+            simpl in J'.
+            apply HeqR.
+            rewrite_env ((getPhiNodesIDs ps1 ++ getCmdsIDs cs1)++getArgsIDs a).
+            apply in_or_app; auto.       
+          apply wf_defs_elim with (id1:=vid) in Hinscope; auto.
+          destruct Hinscope as [? [gv1 [? [Hinscope ?]]]].
+          exists gv1. auto.
+
+        SCase "l3<>l1".
+          assert (In l3 (ListSet.set_diff eq_atom_dec bs_contents [l1])) as G.
+            apply ListSet.set_diff_intro; auto.
+              simpl. intro JJ. destruct JJ as [JJ | JJ]; auto.
+          assert (
+            lookupBlockViaLabelFromFdef 
+              (fdef_intro (fheader_intro f t2 i0 a v) b) l3 = 
+              ret block_intro l3 p c t1) as J1.
+            clear - Hlkvb HuniqF.
+            apply lookupBlockViaIDFromFdef__blockInFdefB in Hlkvb.
+            apply blockInFdefB_lookupBlockViaLabelFromFdef in Hlkvb; auto.
+          destruct HeqR as [_ [HeqR _]].
+          apply HeqR in J1; auto.
+          assert (In vid t) as InVid.
+            clear - J1 HeqR Hlkb1 J3 Hlkvb HbInF HuniqF.
+            apply J1.
+            apply lookupBlockViaIDFromFdef__InGetBlockIDs in Hlkvb; auto.
+          apply wf_defs_elim with (id1:=vid) in Hinscope; auto.
+          destruct Hinscope as [? [gv1 [? [Hinscope ?]]]].
+          exists gv1. auto.
+        Unfocus.
+  
+      destruct J1 as [gv1 J1].
+      simpl. rewrite J1.
+      apply IHps2 in H7.
+        destruct H7 as [RVs H7].
+        rewrite H7. 
+        remember (isPointerTypB t0) as R.
+        destruct R; eauto.
+          inv HwfV. 
+          destruct t0; try solve [inversion HeqR0].
+          assert(exists md, lookupAL metadata rm vid = Some md) as J2.
+            eapply Hwfm; eauto.
+          destruct J2 as [md J2].
+          rewrite J2. eauto.
+  
+        destruct Hin as [ps3 Hin]. subst.
+        exists (ps3++[insn_phi i0 t0 l2]).
+        simpl_env. auto.
+  
+    Case "vc".
+      simpl. inv HwfV.
+      destruct (@const2GV_isnt_stuck (los,nts) s M gl vc t0); auto.
+      rewrite H.
+      apply IHps2 in H7; eauto.
+        destruct H7 as [RVs H7].
+        rewrite H7. 
+        remember (get_const_metadata vc) as R.
+        destruct R as [[[bc ec] tc]|].
+          eapply get_const_metadata_isnt_stuck in H; eauto.
+          destruct H as [gvb [gve [Hc1 Hc2]]].
+          rewrite Hc1. rewrite Hc2. simpl.
+          destruct (isPointerTypB t0); eauto.
+
+          destruct (isPointerTypB t0); eauto.
+  
+        destruct Hin as [ps3 Hin]. subst.
+        exists (ps3++[insn_phi i0 t0 l2]).
+        simpl_env. auto.
+Qed.
+
+Lemma params2GVs_isnt_stuck : forall
+  p22
+  (s : system)
+  los nts
+  (ps : list product)
+  (f : fdef)
+  (i0 : id)
+  n c t v p2
+  (cs : list cmd)
+  (tmn : terminator)
+  (lc : GVMap)
+  (gl : GVMap)
+  (M : mem)
+  (Hwfg1 : wf_global s gl)
+  (HwfSys1 : wf_system nil s)
+  (HmInS1 : moduleInSystemB (module_intro los nts ps) s = true)
+  (HfInPs : InProductsB (product_fdef f) ps = true)
+  (l1 : l)
+  (ps1 : phinodes)
+  (cs1 : list cmd)
+  (Hreach : isReachableFromEntry f
+             (block_intro l1 ps1 (cs1 ++ insn_call i0 n c t v p2 :: cs) tmn))
+  (HbInF : blockInFdefB
+            (block_intro l1 ps1 (cs1 ++ insn_call i0 n c t v p2 :: cs) tmn) f =
+          true)
+  (l0 : list atom)
+  (HeqR : ret l0 =
+         inscope_of_cmd f
+           (block_intro l1 ps1 (cs1 ++ insn_call i0 n c t v p2 :: cs) tmn)
+           (insn_call i0 n c t v p2))
+  (Hinscope : wf_defs f lc l0)
+  rm (Hwfm : wf_rmap f lc rm)
+  (Hex : exists p21, p2 = p21 ++ p22),
+  exists gvs, params2GVs (los, nts) M p22 lc gl rm = Some gvs.
+Proof.
+  induction p22; intros; simpl; eauto.
+
+    destruct a.
+    destruct Hex as [p21 Hex]; subst.
+    assert (exists gv, getOperandValue (los, nts) M v0 lc gl = Some gv) as J.
+      eapply getOperandValue_inCmdOps_isnt_stuck; eauto.
+        simpl. unfold valueInParams. right. 
+        assert (J:=@in_split_r _ _ (p21 ++ (t0, v0) :: p22) (t0, v0)).
+        remember (split (p21 ++ (t0, v0) :: p22)) as R.
+        destruct R.
+        simpl in J. apply J.
+        apply In_middle.
+    destruct J as [gv J]. 
+    rewrite J.         
+    eapply IHp22 with (M:=M) in HbInF; eauto.  
+      destruct HbInF as [vidxs HbInF].
+      rewrite HbInF.
+      remember (isPointerTypB t0) as R.
+      destruct R; eauto.
+
+      exists (p21 ++ [(t0,v0)]). simpl_env. auto.
+Qed.
+
+Lemma progress : forall S1,
+  wf_State S1 -> 
+  SBopsem.ds_isFinialState S1 = true \/ 
+  (exists S2, exists tr, SBopsem.dsInsn S1 S2 tr) \/
+  undefined_state S1.
+Proof.
+  intros S1 HwfS1.
+  destruct S1 as [s [los nts] ps ecs gl fs M].
+  destruct HwfS1 as [Hwfg1 [HwfSys1 [HmInS1 HwfECs]]].
+  destruct ecs; try solve [inversion HwfECs].
+  destruct e as [f b cs tmn lc rm als].
+  destruct HwfECs as [[Hreach [HbInF [HfInPs [Hinscope [Hwfm 
+                        [l1 [ps1 [cs1 Heq]]]]]]]]
+                      [HwfECs HwfCall]].
+  subst b.
+  destruct cs.
+  Case "cs=nil".
+    remember (inscope_of_tmn f (block_intro l1 ps1 (cs1 ++ nil) tmn) tmn) as R.
+    destruct R; try solve [inversion Hinscope].
+    destruct tmn.
+    SCase "tmn=ret".
+      simpl in HwfCall.
+      destruct ecs.
+        simpl; auto.      
+
+        right.
+        destruct e as [f' b' cs' tmn' lc' rm' als'].
+        assert (J:=HbInF).
+        apply HwfCall in J. clear HwfCall.
+        destruct cs'; try solve [inversion J].
+        destruct c; try solve [inversion J]. clear J.
+        remember (free_allocas (los,nts) M als) as Rm.
+        destruct Rm as [M' |]; try solve [undefbehave].
+        left. symmetry in HeqRm.
+        rename HeqRm into J.
+        assert (exists lc'', exists rm'', SBopsem.returnUpdateLocals (los,nts) 
+            M' (insn_call i1 n c t0 v0 p) v lc lc' rm rm' gl = Some (lc'',rm'')) 
+            as Hretup.
+          unfold SBopsem.returnUpdateLocals.
+          destruct n; eauto.
+          assert (exists gv : GenericValue, 
+            getOperandValue (los, nts) M' v lc gl = ret gv) as H.
+            eapply getOperandValue_inTmnOperans_isnt_stuck; eauto.
+              simpl. auto.
+          destruct H as [gv H]. rewrite H.
+          destruct t0; eauto.
+          destruct t0; eauto.
+          unfold SBopsem.prop_reg_metadata.            
+          destruct (SBopsem.get_reg_metadata (los, nts) M' gl rm v) as 
+            [[md ?]|]; eauto.
+         
+        destruct Hretup as [lc'' [rm'' Hretup]].
+        exists (SBopsem.mkState s (los, nts) ps 
+           ((SBopsem.mkEC f' b' cs' tmn' lc'' rm'' als')::ecs) gl fs M' Mmap0).
+        exists trace_nil.
+        eauto. 
+
+    SCase "tmn=ret void".
+      simpl in HwfCall.
+      destruct ecs.
+        simpl; auto.      
+
+        right.
+        destruct e as [f' b' cs' tmn' lc' rm' als'].
+        assert (J:=HbInF).
+        apply HwfCall in J. clear HwfCall.
+        destruct cs'; try solve [inversion J].
+        destruct c; try solve [inversion J]. clear J.
+        remember (free_allocas (los,nts) M als) as Rm.
+        destruct Rm as [M' |]; try solve [undefbehave].
+        symmetry in HeqRm.
+        rename HeqRm into J.
+        destruct n; try solve [undefbehave].
+        left.
+        exists (SBopsem.mkState s (los, nts) ps 
+          ((SBopsem.mkEC f' b' cs' tmn' lc' rm' als')::ecs) gl fs M' Mmap0).
+        exists trace_nil.
+        eauto.  
+
+    SCase "tmn=br".
+      right. left.
+      assert (uniqFdef f) as HuniqF.
+        eapply wf_system__uniqFdef; eauto.
+      assert (exists c, getOperandValue (los,nts) M v lc gl = Some c) as Hget.
+        eapply getOperandValue_inTmnOperans_isnt_stuck; eauto.
+          simpl. auto.
+      destruct Hget as [c Hget].
+      assert (exists l', exists ps', exists cs', exists tmn',
+              Some (block_intro l' ps' cs' tmn') = 
+              (if isGVZero (los,nts) c
+                 then lookupBlockViaLabelFromFdef f l3
+                 else lookupBlockViaLabelFromFdef f l2)) as HlkB.
+        eapply wf_system__wf_tmn in HbInF; eauto.
+        inv HbInF. 
+        destruct block1 as [l2' ps2 cs2 tmn2].
+        destruct block2 as [l3' ps3 cs3 tmn3].
+        destruct (isGVZero (los, nts) c).
+          exists l3'. exists ps3. exists cs3. exists tmn3.
+          rewrite H11. auto.
+
+          exists l2'. exists ps2. exists cs2. exists tmn2.
+          rewrite H10. auto.
+
+      destruct HlkB as [l' [ps' [cs' [tmn' HlkB]]]].
+      assert (exists lc', exists rm', SBopsem.switchToNewBasicBlock (los, nts) M
+        (block_intro l' ps' cs' tmn') 
+        (block_intro l1 ps1 (cs1++nil) (insn_br i0 v l2 l3)) gl lc rm = 
+          Some (lc', rm')) as Hswitch.
+         assert (exists RVs, 
+           SBopsem.getIncomingValuesForBlockFromPHINodes (los, nts) M ps'
+             (block_intro l1 ps1 (cs1++nil) (insn_br i0 v l2 l3)) gl lc rm =
+           Some RVs) as J.
+           assert (HwfB := HbInF).
+           eapply wf_system__blockInFdefB__wf_block in HwfB; eauto.
+           simpl_env in *.
+           destruct (isGVZero (los, nts) c).
+             assert (J:=HlkB).
+             symmetry in J.
+             apply lookupBlockViaLabelFromFdef_inv in J; auto.
+             destruct J as [Heq J]; subst.
+             eapply wf_system__lookup__wf_block in HlkB; eauto.
+             inv HlkB. clear H9 H10.
+             eapply wf_phinodes__getIncomingValuesForBlockFromPHINodes 
+               with (ps':=ps')(cs':=cs')(tmn':=tmn')(l0:=l'); eauto.
+               apply reachable_successors with (l0:=l1)(cs:=ps1)(ps:=cs1)
+                 (tmn:=insn_br i0 v l2 l'); simpl; auto.
+               simpl. auto.    
+               exists nil. auto.
+
+             assert (J:=HlkB).
+             symmetry in J.
+             apply lookupBlockViaLabelFromFdef_inv in J; auto.
+             destruct J as [Heq J]; subst.
+             eapply wf_system__lookup__wf_block in HlkB; eauto.
+             inv HlkB. clear H9 H10.
+             eapply wf_phinodes__getIncomingValuesForBlockFromPHINodes 
+               with (ps':=ps')(cs':=cs')(tmn':=tmn')(l0:=l'); eauto.
+               apply reachable_successors with (l0:=l1)(cs:=ps1)(ps:=cs1)
+                 (tmn:=insn_br i0 v l' l3); simpl; auto.
+               simpl. auto.    
+               exists nil. auto.
+         
+         destruct J as [RVs J].
+         unfold switchToNewBasicBlock. simpl.
+         rewrite J. destruct (updateValuesForNewBlock RVs lc rm); eauto.
+
+      destruct Hswitch as [lc' [rm' Hswitch]].
+      exists (mkState s (los, nts) ps 
+              ((mkEC f (block_intro l' ps' cs' tmn') cs' tmn' lc' rm' als)
+              ::ecs) gl fs M Mmap0).
+      exists trace_nil. eauto.
+
+    SCase "tmn=br_uncond".
+      right. left.
+      assert (uniqFdef f) as HuniqF.
+        eapply wf_system__uniqFdef; eauto.
+      assert (exists ps', exists cs', exists tmn',
+        Some (block_intro l2 ps' cs' tmn') = lookupBlockViaLabelFromFdef f l2) 
+          as HlkB.
+        eapply wf_system__wf_tmn in HbInF; eauto.
+        inv HbInF.        
+        exists ps1. exists (cs1++nil). exists (insn_br_uncond i0 l2).
+        rewrite H6. 
+        apply lookupBlockViaLabelFromFdef_inv in H6; auto.
+        destruct H6 as [H6 _]; subst. auto.
+
+      destruct HlkB as [ps' [cs' [tmn' HlkB]]].
+
+      assert (exists lc', exists rm', switchToNewBasicBlock (los, nts) M
+        (block_intro l2 ps' cs' tmn') 
+        (block_intro l1 ps1 (cs1 ++ nil) (insn_br_uncond i0 l2)) gl lc rm = 
+          Some (lc', rm')) as Hswitch.
+         assert (exists RVs, 
+           getIncomingValuesForBlockFromPHINodes (los, nts) M ps'
+             (block_intro l1 ps1 (cs1 ++ nil) (insn_br_uncond i0 l2)) gl lc rm =
+           Some RVs) as J.
+           assert (HwfB := HbInF).
+           eapply wf_system__blockInFdefB__wf_block in HwfB; eauto.
+           eapply wf_system__lookup__wf_block in HlkB; eauto.
+           inv HlkB. clear H9 H10.
+           eapply wf_phinodes__getIncomingValuesForBlockFromPHINodes 
+             with (l0:=l2); eauto.      
+             apply reachable_successors with (l0:=l1)(cs:=ps1)(ps:=cs1++nil)
+               (tmn:=insn_br_uncond i0 l2); simpl; auto.
+             simpl. auto.
+             exists nil. auto.
+         
+         destruct J as [RVs J].
+         unfold switchToNewBasicBlock. simpl.
+         rewrite J. 
+         destruct (updateValuesForNewBlock RVs lc rm). eauto.
+
+      destruct Hswitch as [lc' [rm' Hswitch]].
+      exists (mkState s (los, nts) ps 
+              ((mkEC f (block_intro l2 ps' cs' tmn') cs' tmn' lc' rm' als)
+              ::ecs) gl fs M Mmap0).
+      exists trace_nil. eauto.
+
+    SCase "tmn=unreachable".
+      undefbehave.
+
+  Case "cs<>nil".
+    assert (wf_insn nil s (module_intro los nts ps) f 
+      (block_intro l1 ps1 (cs1 ++ c :: cs) tmn) (insn_cmd c)) as Hwfc.
+      assert (In c (cs1++c::cs)) as H. 
+        apply in_or_app. simpl. auto.
+      eapply wf_system__wf_cmd with (c:=c) in HbInF; eauto.
+    remember (inscope_of_cmd f (block_intro l1 ps1 (cs1 ++ c :: cs) tmn) c) as R.
+    destruct R; try solve [inversion Hinscope].
+    right.
+    destruct c.
+  SCase "c=bop". 
+    left.
+    assert (exists gv3, BOP (los,nts) M lc gl b s0 v v0 = Some gv3) as Hinsn_bop.
+      unfold BOP.      
+      assert (exists gv, getOperandValue (los, nts) M v lc gl = Some gv) as J.
+        eapply getOperandValue_inCmdOps_isnt_stuck; eauto.
+          simpl; auto.
+      assert (exists gv, getOperandValue (los, nts) M v0 lc gl = Some gv) as J0.
+        eapply getOperandValue_inCmdOps_isnt_stuck; eauto.
+          simpl; auto.
+          destruct J as [gv J].
+      destruct J0 as [gv0 J0].
+      rewrite J. rewrite J0. 
+      unfold mbop. 
+      destruct (GV2val (los, nts) gv); eauto.
+      destruct v1; eauto.
+      destruct (GV2val (los, nts) gv0); eauto.
+      destruct v1; eauto.
+      destruct (eq_nat_dec (wz + 1) (Size.to_nat s0)); eauto.
+      destruct b; eauto.
+    destruct Hinsn_bop as [gv3 Hinsn_bop].
+    exists 
+         {|
+         SBopsem.CurSystem := s;
+         SBopsem.CurTargetData := (los, nts);
+         SBopsem.CurProducts := ps;
+         SBopsem.ECS := {|
+                SBopsem.CurFunction := f;
+                SBopsem.CurBB := block_intro l1 ps1
+                           (cs1 ++ insn_bop i0 b s0 v v0 :: cs) tmn;
+                SBopsem.CurCmds := cs;
+                SBopsem.Terminator := tmn;
+                SBopsem.Locals := (updateAddAL _ lc i0 gv3);
+                SBopsem.Rmap := rm;
+                SBopsem.Allocas := als |} :: ecs;
+         SBopsem.Globals := gl;
+         SBopsem.FunTable := fs;
+         SBopsem.Mem := M;
+         SBopsem.Mmap := Mmap0 |}.
+     exists trace_nil. eauto.
+
+  SCase "c=fbop". 
+    left.
+    assert (exists gv3, FBOP (los,nts) M lc gl f0 f1 v v0 = Some gv3) 
+      as Hinsn_fbop.
+      unfold FBOP.      
+      assert (exists gv, getOperandValue (los, nts) M v lc gl = Some gv) as J.
+        eapply getOperandValue_inCmdOps_isnt_stuck; eauto.
+          simpl; auto.
+      assert (exists gv, getOperandValue (los, nts) M v0 lc gl = Some gv) as J0.
+        eapply getOperandValue_inCmdOps_isnt_stuck; eauto.
+          simpl; auto.
+      destruct J as [gv J].
+      destruct J0 as [gv0 J0].
+      rewrite J. rewrite J0. 
+      unfold mfbop. 
+      destruct (GV2val (los, nts) gv); eauto.
+      destruct v1; eauto.
+      destruct (GV2val (los, nts) gv0); eauto.
+      destruct v1; eauto.
+      inv Hwfc.
+      apply wf_value__wf_typ in H7.
+      destruct H7 as [J1 J2].
+      destruct f1; try solve [eauto | inversion J1].
+
+    destruct Hinsn_fbop as [gv3 Hinsn_fbop].
+    exists 
+         {|
+         SBopsem.CurSystem := s;
+         SBopsem.CurTargetData := (los, nts);
+         SBopsem.CurProducts := ps;
+         SBopsem.ECS := {|
+                SBopsem.CurFunction := f;
+                SBopsem.CurBB := block_intro l1 ps1
+                           (cs1 ++ insn_fbop i0 f0 f1 v v0 :: cs) tmn;
+                SBopsem.CurCmds := cs;
+                SBopsem.Terminator := tmn;
+                SBopsem.Locals := (updateAddAL _ lc i0 gv3);
+                SBopsem.Rmap := rm;
+                SBopsem.Allocas := als |} :: ecs;
+         SBopsem.Globals := gl;
+         SBopsem.FunTable := fs;
+         SBopsem.Mem := M;
+         SBopsem.Mmap := Mmap0 |}.
+     exists trace_nil. eauto.
+
+  SCase "c=extractvalue".
+    left.
+    assert (exists gv, getOperandValue (los, nts) M v lc gl = Some gv) as J.
+      eapply getOperandValue_inCmdOps_isnt_stuck; eauto.
+        simpl; auto.
+    destruct J as [gv J].
+    assert (exists gv', extractGenericValue (los, nts) t gv l2 = Some gv') as J'.
+      unfold extractGenericValue.
+      destruct (intConsts2Nats (los, nts) l2); eauto.
+      destruct (mgetoffset (los, nts) t l3); eauto.
+      destruct (mget (los, nts) gv i1 t); eauto.
+    destruct J' as [gv' J'].
+    exists {|
+         SBopsem.CurSystem := s;
+         SBopsem.CurTargetData := (los, nts);
+         SBopsem.CurProducts := ps;
+         SBopsem.ECS := {|
+                SBopsem.CurFunction := f;
+                SBopsem.CurBB := block_intro l1 ps1
+                           (cs1 ++ insn_extractvalue i0 t v l2 :: cs) tmn;
+                SBopsem.CurCmds := cs;
+                SBopsem.Terminator := tmn;
+                SBopsem.Locals := (updateAddAL _ lc i0 gv');
+                SBopsem.Rmap := rm;
+                SBopsem.Allocas := als |} :: ecs;
+         SBopsem.Globals := gl;
+         SBopsem.FunTable := fs;
+         SBopsem.Mem := M;
+         SBopsem.Mmap := Mmap0|}.
+     exists trace_nil. eauto.
+
+  SCase "c=insertvalue".
+    left.
+    assert (exists gv, getOperandValue (los, nts) M v lc gl = Some gv) as J.
+      eapply getOperandValue_inCmdOps_isnt_stuck; eauto.
+        simpl; auto.
+    destruct J as [gv J].
+    assert (exists gv', getOperandValue (los, nts) M v0 lc gl = Some gv') as J'.
+      eapply getOperandValue_inCmdOps_isnt_stuck; eauto.
+        simpl; auto.
+    destruct J' as [gv' J'].
+    assert (exists gv'', insertGenericValue (los, nts) t gv l2 t0 gv' = 
+      Some gv'') as J''.
+      unfold insertGenericValue.
+      destruct (intConsts2Nats (los, nts) l2); eauto.
+      destruct (mgetoffset (los, nts) t l3); eauto.
+      destruct (mset (los, nts) gv i1 t0 gv'); eauto.
+    destruct J'' as [gv'' J''].
+    exists 
+         {|
+         SBopsem.CurSystem := s;
+         SBopsem.CurTargetData := (los, nts);
+         SBopsem.CurProducts := ps;
+         SBopsem.ECS := {|
+                SBopsem.CurFunction := f;
+                SBopsem.CurBB := block_intro l1 ps1
+                           (cs1 ++ insn_insertvalue i0 t v t0 v0 l2 :: cs) tmn;
+                SBopsem.CurCmds := cs;
+                SBopsem.Terminator := tmn;
+                SBopsem.Locals := (updateAddAL _ lc i0 gv'');
+                SBopsem.Rmap := rm;
+                SBopsem.Allocas := als |} :: ecs;
+         SBopsem.Globals := gl;
+         SBopsem.FunTable := fs;
+         SBopsem.Mem := M;
+         SBopsem.Mmap := Mmap0 |}.
+     exists trace_nil. eauto.
+
+  SCase "c=malloc". 
+    inv Hwfc. inv H12.
+    apply feasible_typ_inv in H.
+    destruct H as [ssz [asz [J1 J2]]].
+    assert (exists gv, getOperandValue (los, nts) M v lc gl = Some gv) as J.
+      eapply getOperandValue_inCmdOps_isnt_stuck; eauto.
+        simpl; auto.
+    destruct J as [gv J].
+    remember (malloc (los, nts) M asz gv a) as R.
+    destruct R as [[M' mb] |].
+      left.
+      assert (exists n, GV2int (los, nts) Size.ThirtyTwo gv = Some n) as H.
+        clear - HeqR0. unfold malloc in HeqR0.
+        destruct (GV2int (los, nts) Size.ThirtyTwo gv); inv HeqR0; eauto.
+      destruct H as [n H].
+      remember (prop_reg_metadata lc rm i0 (blk2GV (los, nts) mb) 
+        (mkMD (base2GV (los, nts) mb) (bound2GV (los, nts) mb asz n))) as R.
+      destruct R as [lc' rm'].
+      exists 
+         {|
+         SBopsem.CurSystem := s;
+         SBopsem.CurTargetData := (los, nts);
+         SBopsem.CurProducts := ps;
+         SBopsem.ECS := {|
+                SBopsem.CurFunction := f;
+                SBopsem.CurBB := block_intro l1 ps1
+                           (cs1 ++ insn_malloc i0 t v a :: cs) tmn;
+                SBopsem.CurCmds := cs;
+                SBopsem.Terminator := tmn;
+                SBopsem.Locals := lc';
+                SBopsem.Rmap := rm';
+                SBopsem.Allocas := als |} :: ecs;
+         SBopsem.Globals := gl;
+         SBopsem.FunTable := fs;
+         SBopsem.Mem := M';
+         SBopsem.Mmap := Mmap0 |}.
+      exists trace_nil.
+      eauto.
+      
+      unfold undefined_state.
+      right. rewrite J. rewrite J2. rewrite <- HeqR0. undefbehave.
+
+  SCase "free". 
+    assert (exists gv, getOperandValue (los, nts) M v lc gl = Some gv) as J.
+      eapply getOperandValue_inCmdOps_isnt_stuck; eauto.
+        simpl; auto.
+    destruct J as [gv J].
+    remember (free (los, nts) M gv) as R.
+    destruct R as [M'|].
+      left.
+      exists 
+         {|
+         SBopsem.CurSystem := s;
+         SBopsem.CurTargetData := (los, nts);
+         SBopsem.CurProducts := ps;
+         SBopsem.ECS := {|
+                SBopsem.CurFunction := f;
+                SBopsem.CurBB := block_intro l1 ps1
+                           (cs1 ++ insn_free i0 t v :: cs) tmn;
+                SBopsem.CurCmds := cs;
+                SBopsem.Terminator := tmn;
+                SBopsem.Locals := lc;
+                SBopsem.Rmap := rm;
+                SBopsem.Allocas := als |} :: ecs;
+         SBopsem.Globals := gl;
+         SBopsem.FunTable := fs;
+         SBopsem.Mem := M';
+         SBopsem.Mmap := Mmap0 |}.
+      exists trace_nil.
+      eauto.      
+      
+      unfold undefined_state.
+      right. rewrite J. rewrite <- HeqR0. undefbehave.
+
+  SCase "alloca".
+    inv Hwfc. inv H12.
+    apply feasible_typ_inv in H.
+    destruct H as [ssz [asz [J1 J2]]].
+    assert (exists gv, getOperandValue (los, nts) M v lc gl = Some gv) as J.
+      eapply getOperandValue_inCmdOps_isnt_stuck; eauto.
+        simpl; auto.
+    destruct J as [gv J].
+    remember (malloc (los, nts) M asz gv a) as R.
+    destruct R as [[M' mb] |].
+      assert (exists n, GV2int (los, nts) Size.ThirtyTwo gv = Some n) as H.
+        clear - HeqR0. unfold malloc in HeqR0.
+        destruct (GV2int (los, nts) Size.ThirtyTwo gv); inv HeqR0; eauto.
+      destruct H as [n H].
+      remember (prop_reg_metadata lc rm i0 (blk2GV (los, nts) mb) 
+        (mkMD (base2GV (los, nts) mb) (bound2GV (los, nts) mb asz n))) as R.
+      destruct R as [lc' rm'].
+      left.
+      exists 
+         {|
+         SBopsem.CurSystem := s;
+         SBopsem.CurTargetData := (los, nts);
+         SBopsem.CurProducts := ps;
+         SBopsem.ECS := {|
+                SBopsem.CurFunction := f;
+                SBopsem.CurBB := block_intro l1 ps1
+                           (cs1 ++ insn_alloca i0 t v a :: cs) tmn;
+                SBopsem.CurCmds := cs;
+                SBopsem.Terminator := tmn;
+                SBopsem.Locals := lc';
+                SBopsem.Rmap := rm';
+                SBopsem.Allocas := (mb::als) |} :: ecs;
+         SBopsem.Globals := gl;
+         SBopsem.FunTable := fs;
+         SBopsem.Mem := M';
+         SBopsem.Mmap := Mmap0 |}.
+      exists trace_nil.
+      eauto.
+      
+      right.
+      unfold undefined_state.
+      right. rewrite J. rewrite J2. rewrite <- HeqR0. undefbehave.
+
+  SCase "load".
+    assert (exists gv, getOperandValue (los, nts) M v lc gl = Some gv) as J.
+      eapply getOperandValue_inCmdOps_isnt_stuck; eauto.
+        simpl; auto.
+    destruct J as [gv J].
+    remember (mload (los, nts) M gv t a) as R.
+    destruct R as [gv'|].
+    SSCase "load ok".
+      assert (exists omd, SBopsem.get_reg_metadata (los, nts) M gl rm v = 
+        Some omd) as J2.
+        clear - Hwfm J HbInF Hwfc.
+        destruct v; simpl in *.
+          assert (exists md, lookupAL metadata rm i1 = Some md) as J0.
+            eapply Hwfm with (t1:=t); eauto.
+              inv Hwfc. inv H6; auto.
+          destruct J0 as [md J0].
+          rewrite J0; eauto.
+
+          remember (get_const_metadata c) as R.
+          destruct R as [[[bc ec] tc]|]; eauto.
+            eapply get_const_metadata_isnt_stuck in J; eauto.
+            destruct J as [gvb [gve [Hc1 Hc2]]].
+            rewrite Hc1. rewrite Hc2. simpl.
+            eauto.
+      destruct J2 as [[md mt] J2].
+      destruct (assert_mptr_dec (los, nts) t gv md) as [J3 | J3].
+      SSSCase "assert ok".
+        remember (isPointerTypB t) as R1.
+        destruct R1.      
+          SSSSCase "load_ptr".
+          remember (SBopsem.prop_reg_metadata lc rm i0 gv' 
+            (SBopsem.get_mem_metadata (los, nts) Mmap0 gv)) as R.
+          destruct R as [lc' rm'].
+          left.
+          exists 
+           {|
+             SBopsem.CurSystem := s;
+             SBopsem.CurTargetData := (los, nts);
+             SBopsem.CurProducts := ps;
+             SBopsem.ECS := {|
+                SBopsem.CurFunction := f;
+                SBopsem.CurBB := block_intro l1 ps1
+                           (cs1 ++ insn_load i0 t v a :: cs) tmn;
+                SBopsem.CurCmds := cs;
+                SBopsem.Terminator := tmn;
+                SBopsem.Locals := lc';
+                SBopsem.Rmap := rm';
+                SBopsem.Allocas := als |} :: ecs;
+             SBopsem.Globals := gl;
+             SBopsem.FunTable := fs;
+             SBopsem.Mem := M;
+             SBopsem.Mmap := Mmap0 |}.
+          exists trace_nil. eauto.
+
+          SSSSCase "load_nptr".
+          left.
+          exists 
+           {|
+             SBopsem.CurSystem := s;
+             SBopsem.CurTargetData := (los, nts);
+             SBopsem.CurProducts := ps;
+             SBopsem.ECS := {|
+                SBopsem.CurFunction := f;
+                SBopsem.CurBB := block_intro l1 ps1
+                           (cs1 ++ insn_load i0 t v a :: cs) tmn;
+                SBopsem.CurCmds := cs;
+                SBopsem.Terminator := tmn;
+                SBopsem.Locals := updateAddAL _ lc i0 gv';
+                SBopsem.Rmap := rm;
+                SBopsem.Allocas := als |} :: ecs;
+             SBopsem.Globals := gl;
+             SBopsem.FunTable := fs;
+             SBopsem.Mem := M;
+             SBopsem.Mmap := Mmap0 |}.
+          exists trace_nil. eauto.
+
+      SSSCase "assert fails".
+        right.
+        unfold undefined_state. unfold memory_violation.
+        right. rewrite J. rewrite J2. undefbehave.
+
+    SSCase "load fails".
+      right.
+      unfold undefined_state.
+      right. rewrite J. rewrite <- HeqR0. undefbehave.
+
+  SCase "store".
+    assert (exists gv, getOperandValue (los, nts) M v lc gl = Some gv) as J.
+      eapply getOperandValue_inCmdOps_isnt_stuck; eauto.
+        simpl; auto.
+    destruct J as [gv J].
+    assert (exists gv, getOperandValue (los, nts) M v0 lc gl = Some gv) as J0.
+      eapply getOperandValue_inCmdOps_isnt_stuck; eauto.
+        simpl; auto.
+    destruct J0 as [mgv J0].
+    remember (mstore (los, nts) M mgv t gv a) as R.
+    destruct R as [M'|].
+    SSCase "store ok".
+      assert (exists omd, SBopsem.get_reg_metadata (los, nts) M gl rm v0 = 
+        Some omd) as J2.
+        clear - Hwfm J0 HbInF Hwfc.
+        destruct v0; simpl in *.
+          assert (exists md, lookupAL metadata rm i1 = Some md) as J1.
+            eapply Hwfm with (t1:=t); eauto.
+              inv Hwfc. inv H10; eauto.
+          destruct J1 as [md J1].
+          rewrite J1; eauto.
+
+          remember (get_const_metadata c) as R.
+          destruct R as [[[bc ec] tc]|]; eauto.
+            eapply get_const_metadata_isnt_stuck in J0; eauto.
+            destruct J0 as [gvb [gve [Hc1 Hc2]]].
+            rewrite Hc1. rewrite Hc2. simpl.
+            eauto.
+      destruct J2 as [[md mt] J2].
+      destruct (assert_mptr_dec (los, nts) t mgv md) as [J3 | J3].
+      SSSCase "assert ok".
+        remember (isPointerTypB t) as R1.
+        destruct R1.      
+        SSSSCase "store_ptr".
+          assert (exists omd, SBopsem.get_reg_metadata (los, nts) M gl rm v = 
+            Some omd) as J4.
+            clear - Hwfm J HbInF Hwfc HeqR1.
+            destruct v; simpl in *.
+              assert (exists md, lookupAL metadata rm i1 = Some md) as J1.
+                destruct t; try solve [inversion HeqR1].
+                eapply Hwfm with (t1:=t); eauto.
+                  inv Hwfc. inv H7; eauto.
+              destruct J1 as [md J1].
+              rewrite J1; eauto.
+
+              remember (get_const_metadata c) as R.
+              destruct R as [[[bc ec] tc]|]; eauto.
+                eapply get_const_metadata_isnt_stuck in J; eauto.
+                destruct J as [gvb [gve [Hc1 Hc2]]].
+                rewrite Hc1. rewrite Hc2. simpl.
+                eauto.
+          destruct J4 as [[md' mt'] J4].
+          left.
+          remember (set_mem_metadata (los, nts) Mmap0 mgv md') as Mmap0'.
+          exists 
+             {|
+             CurSystem := s;
+             CurTargetData := (los, nts);
+             CurProducts := ps;
+             ECS := {|
+                    CurFunction := f;
+                    CurBB := block_intro l1 ps1
+                               (cs1 ++ insn_store i0 t v v0 a :: cs) tmn;
+                    CurCmds := cs;
+                    Terminator := tmn;
+                    Locals := lc;
+                    Rmap := rm;
+                    Allocas := als |} :: ecs;
+             Globals := gl;
+             FunTable := fs;
+             Mem := M';
+             Mmap := Mmap0'|}.
+          exists trace_nil.
+          eauto.
+
+        SSSSCase "store_nptr".
+          left.
+          exists 
+             {|
+             CurSystem := s;
+             CurTargetData := (los, nts);
+             CurProducts := ps;
+             ECS := {|
+                    CurFunction := f;
+                    CurBB := block_intro l1 ps1
+                               (cs1 ++ insn_store i0 t v v0 a :: cs) tmn;
+                    CurCmds := cs;
+                    Terminator := tmn;
+                    Locals := lc;
+                    Rmap := rm;
+                    Allocas := als |} :: ecs;
+             Globals := gl;
+             FunTable := fs;
+             Mem := M';
+             Mmap := Mmap0|}.
+          exists trace_nil.
+          eauto.
+
+      SSSCase "assert fails".
+        right.
+        unfold undefined_state. unfold memory_violation.
+        right. rewrite J0. rewrite J2. undefbehave.
+
+    SSCase "store fails".
+      right.
+      unfold undefined_state.
+      right. rewrite J. rewrite J0. rewrite <- HeqR0. undefbehave.
+
+  SCase "gep".
+    assert (exists gv, getOperandValue (los, nts) M v lc gl = Some gv) as J.
+      eapply getOperandValue_inCmdOps_isnt_stuck; eauto.
+        simpl; auto.
+    destruct J as [mp J].
+    assert (exists vidxs, values2GVs (los, nts) M l2 lc gl = Some vidxs) as J2.
+      eapply values2GVs_isnt_stuck; eauto.
+        exists Nil_list_value. auto.
+    destruct J2 as [vidxs J2].
+    assert (exists mp', GEP (los, nts) t mp vidxs i1 = Some mp') as J3.
+      unfold GEP.
+      destruct (GV2ptr (los, nts) (getPointerSize (los, nts)) mp); eauto.
+      destruct (GVs2Nats (los, nts) vidxs); eauto.
+      destruct (mgep (los, nts) t v0 l3); eauto.
+    destruct J3 as [mp' J3].
+    left.
+    assert (exists omd, SBopsem.get_reg_metadata (los, nts) M gl rm v = 
+      Some omd) as J4.
+      clear - Hwfm J HbInF Hwfc.
+      destruct v; simpl in *.
+        assert (exists md, lookupAL metadata rm i2 = Some md) as J0.
+          eapply Hwfm with (t1:=t); eauto.
+            inv Hwfc. inv H9; auto.
+        destruct J0 as [md J0].
+        rewrite J0; eauto.
+
+        remember (get_const_metadata c) as R.
+        destruct R as [[[bc ec] tc]|]; eauto.
+          eapply get_const_metadata_isnt_stuck in J; eauto.
+          destruct J as [gvb [gve [Hc1 Hc2]]].
+          rewrite Hc1. rewrite Hc2. simpl.
+          eauto.
+    destruct J4 as [[md mt] J4].
+    remember (prop_reg_metadata lc rm i0 mp' md) as R.
+    destruct R as [lc' rm'].
+    exists 
+         {|
+         CurSystem := s;
+         CurTargetData := (los, nts);
+         CurProducts := ps;
+         ECS := {|
+                CurFunction := f;
+                CurBB := block_intro l1 ps1
+                           (cs1 ++ insn_gep i0 i1 t v l2 :: cs) tmn;
+                CurCmds := cs;
+                Terminator := tmn;
+                Locals := lc';
+                Rmap := rm';
+                Allocas := als |} :: ecs;
+         Globals := gl;
+         FunTable := fs;
+         Mem := M;
+         Mmap := Mmap0 |}.
+    exists trace_nil. eauto.
+
+  SCase "trunc".
+    left.
+    assert (exists gv2, TRUNC (los,nts) M lc gl t t0 v t1 = Some gv2) 
+      as Hinsn_trunc.
+      unfold TRUNC.      
+      assert (exists gv, getOperandValue (los, nts) M v lc gl = Some gv) as J.
+        eapply getOperandValue_inCmdOps_isnt_stuck; eauto.
+          simpl; auto.
+      destruct J as [gv J].
+      rewrite J.
+      unfold mtrunc. 
+      destruct (GV2val (los, nts) gv); eauto.
+      inv Hwfc. 
+      inv H5; try solve [destruct v0; eauto].
+        rewrite H11.
+        destruct v0; eauto.
+          destruct floating_point2; try solve [eauto | inversion H13].
+    destruct Hinsn_trunc as [gv2 Hinsn_trunc].
+    exists 
+         {|
+         CurSystem := s;
+         CurTargetData := (los, nts);
+         CurProducts := ps;
+         ECS := {|
+                CurFunction := f;
+                CurBB := block_intro l1 ps1
+                           (cs1 ++ insn_trunc i0 t t0 v t1 :: cs) tmn;
+                CurCmds := cs;
+                Terminator := tmn;
+                Locals := (updateAddAL _ lc i0 gv2);
+                Rmap := rm;
+                Allocas := als |} :: ecs;
+         Globals := gl;
+         FunTable := fs;
+         Mem := M;
+         Mmap := Mmap0 |}.
+     exists trace_nil. eauto.
+
+  SCase "ext".
+    left.
+    assert (exists gv2, EXT (los,nts) M lc gl e t v t0 = Some gv2) 
+      as Hinsn_ext.
+      unfold EXT.      
+      assert (exists gv, getOperandValue (los, nts) M v lc gl = Some gv) as J.
+        eapply getOperandValue_inCmdOps_isnt_stuck; eauto.
+          simpl; auto.
+      destruct J as [gv J].
+      rewrite J.
+      unfold mext. 
+      inv Hwfc. 
+      inv H5; try solve 
+        [destruct (GV2val (los, nts) gv); eauto; destruct v0; eauto].
+        rewrite H11.
+        destruct (GV2val (los, nts) gv); eauto; destruct v0; eauto.
+    destruct Hinsn_ext as [gv2 Hinsn_ext].
+    exists 
+         {|
+         CurSystem := s;
+         CurTargetData := (los, nts);
+         CurProducts := ps;
+         ECS := {|
+                CurFunction := f;
+                CurBB := block_intro l1 ps1
+                           (cs1 ++ insn_ext i0 e t v t0 :: cs) tmn;
+                CurCmds := cs;
+                Terminator := tmn;
+                Locals := (updateAddAL _ lc i0 gv2);
+                Rmap := rm;
+                Allocas := als |} :: ecs;
+         Globals := gl;
+         FunTable := fs;
+         Mem := M;
+         Mmap := Mmap0 |}.
+     exists trace_nil. eauto.
+
+  SCase "cast". 
+    left.
+    assert (exists gv, getOperandValue (los, nts) M v lc gl = Some gv) as J.
+      eapply getOperandValue_inCmdOps_isnt_stuck; eauto.
+        simpl; auto.
+    destruct J as [gv J].
+    assert (exists gv2, CAST (los,nts) M lc gl c t v t0 = Some gv2) 
+      as Hinsn_cast.
+      unfold CAST.      
+      rewrite J.
+      unfold mcast, mptrtoint.
+      inv Hwfc. 
+      inv H5; eauto.
+        destruct (GV2val (los, nts) gv); eauto.
+        destruct v0; eauto.
+        destruct (Mem.ptr2int M b 0); eauto.
+
+        destruct (GV2val (los, nts) gv); eauto.
+        destruct v0; eauto.
+        destruct (Mem.int2ptr M (Int.signed wz i1)); eauto.
+        destruct p; eauto.
+
+    destruct Hinsn_cast as [gv2 Hinsn_cast].
+    remember c as c'.
+    destruct c; try solve [
+      exists 
+         {|
+         CurSystem := s;
+         CurTargetData := (los, nts);
+         CurProducts := ps;
+         ECS := {|
+                CurFunction := f;
+                CurBB := block_intro l1 ps1
+                           (cs1 ++ insn_cast i0 c' t v t0 :: cs) tmn;
+                CurCmds := cs;
+                Terminator := tmn;
+                Locals := (updateAddAL _ lc i0 gv2);
+                Rmap := rm;
+                Allocas := als |} :: ecs;
+         Globals := gl;
+         FunTable := fs;
+         Mem := M;
+         Mmap := Mmap0 |};
+       exists trace_nil; subst; eapply dsOtherCast; 
+         try solve [eauto | split; congruence]].
+    SSCase "case_inttoptr".
+      remember (prop_reg_metadata lc rm i0 gv2 (mkMD null null)) as R.
+      destruct R as [lc' rm'].
+      exists 
+         {|
+         CurSystem := s;
+         CurTargetData := (los, nts);
+         CurProducts := ps;
+         ECS := {|
+                CurFunction := f;
+                CurBB := block_intro l1 ps1
+                           (cs1 ++ insn_cast i0 c' t v t0 :: cs) tmn;
+                CurCmds := cs;
+                Terminator := tmn;
+                Locals := lc';
+                Rmap := rm';
+                Allocas := als |} :: ecs;
+         Globals := gl;
+         FunTable := fs;
+         Mem := M;
+         Mmap := Mmap0 |}.
+       exists trace_nil. subst. eauto.
+
+    SSCase "case_bitcast".
+      remember (isPointerTypB t) as R.
+      destruct R.
+      SSSCase "case_ptr".
+
+        assert (exists omd, SBopsem.get_reg_metadata (los, nts) M gl rm v = 
+          Some omd) as J4.
+          clear - Hwfm J HbInF Hwfc HeqR0. 
+          destruct v; simpl in *.
+            assert (exists md, lookupAL metadata rm i1 = Some md) as J0.
+              destruct t; try solve [inversion HeqR0].
+              eapply Hwfm with (t1:=t); eauto.
+                inv Hwfc. 
+                inv H5.
+                  inv H7; auto.
+                  inv H8; auto.
+            destruct J0 as [md J0].
+            rewrite J0; eauto.
+
+            remember (get_const_metadata c) as R.
+            destruct R as [[[bc ec] tc]|]; eauto.
+              eapply get_const_metadata_isnt_stuck in J; eauto.
+              destruct J as [gvb [gve [Hc1 Hc2]]].
+              rewrite Hc1. rewrite Hc2. simpl.
+              eauto.
+        destruct J4 as [[md mt] J4].
+        remember (prop_reg_metadata lc rm i0 gv2 md) as R.
+        destruct R as [lc' rm'].
+        exists 
+           {|
+           CurSystem := s;
+           CurTargetData := (los, nts);
+           CurProducts := ps;
+           ECS := {|
+                CurFunction := f;
+                CurBB := block_intro l1 ps1
+                           (cs1 ++ insn_cast i0 c' t v t0 :: cs) tmn;
+                CurCmds := cs;
+                Terminator := tmn;
+                Locals := lc';
+                Rmap := rm';
+                Allocas := als |} :: ecs;
+           Globals := gl;
+           FunTable := fs;
+           Mem := M;
+           Mmap := Mmap0 |}.
+         exists trace_nil. subst. eauto.
+
+      SSSCase "case_nptr".
+        exists 
+           {|
+           CurSystem := s;
+           CurTargetData := (los, nts);
+           CurProducts := ps;
+           ECS := {|
+                CurFunction := f;
+                CurBB := block_intro l1 ps1
+                           (cs1 ++ insn_cast i0 c' t v t0 :: cs) tmn;
+                CurCmds := cs;
+                Terminator := tmn;
+                Locals := (updateAddAL _ lc i0 gv2);
+                Rmap := rm;
+                Allocas := als |} :: ecs;
+           Globals := gl;
+           FunTable := fs;
+           Mem := M;
+           Mmap := Mmap0 |}.
+         exists trace_nil. subst. eauto.
+
+  SCase "icmp".
+    left.
+    assert (exists gv2, ICMP (los,nts) M lc gl c t v v0 = Some gv2) 
+      as Hinsn_icmp.
+      unfold ICMP.      
+      assert (exists gv, getOperandValue (los, nts) M v lc gl = Some gv) as J.
+        eapply getOperandValue_inCmdOps_isnt_stuck; eauto.
+          simpl; auto.
+      destruct J as [gv J].
+      rewrite J.
+      assert (exists gv, getOperandValue (los, nts) M v0 lc gl = Some gv) as J0.
+        eapply getOperandValue_inCmdOps_isnt_stuck; eauto.
+          simpl; auto.
+      destruct J0 as [gv0 J0].
+      rewrite J0.
+      unfold micmp.
+      inv Hwfc. 
+      unfold isPointerTyp in H11. unfold is_true in H11.
+      unfold micmp_int.
+      destruct H11 as [H11 | H11].
+        destruct t; try solve [simpl in H11; contradict H11; auto].
+        destruct (GV2val (los,nts) gv); eauto.
+        destruct v1; eauto.
+        destruct (GV2val (los,nts) gv0); eauto.
+        destruct v1; eauto.
+        destruct c; eauto.
+
+        destruct t; try solve [simpl in H11; contradict H11; auto].
+        destruct (mptrtoint (los, nts) M gv Size.ThirtyTwo); eauto.
+        destruct (mptrtoint (los, nts) M gv0 Size.ThirtyTwo); eauto.
+        destruct (GV2val (los, nts) g); eauto.
+        destruct v1; eauto.
+        destruct (GV2val (los, nts) g0); eauto.
+        destruct v1; eauto.
+        destruct c; eauto.
+    destruct Hinsn_icmp as [gv2 Hinsn_icmp].
+    exists 
+         {|
+         CurSystem := s;
+         CurTargetData := (los, nts);
+         CurProducts := ps;
+         ECS := {|
+                CurFunction := f;
+                CurBB := block_intro l1 ps1
+                           (cs1 ++ insn_icmp i0 c t v v0 :: cs) tmn;
+                CurCmds := cs;
+                Terminator := tmn;
+                Locals := (updateAddAL _ lc i0 gv2);
+                Rmap := rm;
+                Allocas := als |} :: ecs;
+         Globals := gl;
+         FunTable := fs;
+         Mem := M;
+         Mmap := Mmap0 |}.
+     exists trace_nil. eauto.
+
+  SCase "fcmp".
+    left.
+    assert (exists gv2, FCMP (los,nts) M lc gl f0 f1 v v0 = Some gv2) 
+      as Hinsn_fcmp.
+      unfold FCMP.      
+      assert (exists gv, getOperandValue (los, nts) M v lc gl = Some gv) as J.
+        eapply getOperandValue_inCmdOps_isnt_stuck; eauto.
+          simpl; auto.
+      destruct J as [gv J].
+      rewrite J.
+      assert (exists gv, getOperandValue (los, nts) M v0 lc gl = Some gv) as J0.
+        eapply getOperandValue_inCmdOps_isnt_stuck; eauto.
+          simpl; auto.
+      destruct J0 as [gv0 J0].
+      rewrite J0.
+      unfold mfcmp.
+      inv Hwfc. 
+      destruct (GV2val (los, nts) gv); eauto.
+      destruct v1; eauto.
+      destruct (GV2val (los, nts) gv0); eauto.
+      destruct v1; eauto.
+      apply wf_value__wf_typ in H10.
+      destruct H10 as [J1 J2].
+      destruct f1; try solve [eauto | inversion J1].
+        destruct f0; try solve [eauto | inversion H8].
+        destruct f0; try solve [eauto | inversion H8].
+    destruct Hinsn_fcmp as [gv2 Hinsn_fcmp].
+    exists 
+         {|
+         CurSystem := s;
+         CurTargetData := (los, nts);
+         CurProducts := ps;
+         ECS := {|
+                CurFunction := f;
+                CurBB := block_intro l1 ps1
+                           (cs1 ++ insn_fcmp i0 f0 f1 v v0 :: cs) tmn;
+                CurCmds := cs;
+                Terminator := tmn;
+                Locals := (updateAddAL _ lc i0 gv2);
+                Rmap := rm;
+                Allocas := als |} :: ecs;
+         Globals := gl;
+         FunTable := fs;
+         Mem := M;
+         Mmap := Mmap0 |}.
+     exists trace_nil. eauto.
+
+  SCase "select".
+    assert (exists gv, getOperandValue (los, nts) M v lc gl = Some gv) as J.
+      eapply getOperandValue_inCmdOps_isnt_stuck; eauto.
+        simpl; auto.
+    destruct J as [gv J].
+    assert (exists gv0, getOperandValue (los, nts) M v0 lc gl = Some gv0) as J0.
+      eapply getOperandValue_inCmdOps_isnt_stuck; eauto.
+        simpl; auto.
+    destruct J0 as [gv0 J0].
+    assert (exists gv1, getOperandValue (los, nts) M v1 lc gl = Some gv1) as J1.
+      eapply getOperandValue_inCmdOps_isnt_stuck; eauto.
+        simpl; auto.
+    destruct J1 as [gv1 J1].
+    left.
+    remember (isPointerTypB t) as R.
+    destruct R.
+    SSCase "select_ptr".
+      assert (exists omd, SBopsem.get_reg_metadata (los, nts) M gl rm v0 = 
+          Some omd) as J2.
+        clear - Hwfm J0 HbInF Hwfc HeqR0. 
+        destruct v0; simpl in *.
+          assert (exists md, lookupAL metadata rm i1 = Some md) as J0'.
+            destruct t; try solve [inversion HeqR0].
+            eapply Hwfm with (t1:=t); eauto.
+              inv Hwfc. inv H11; auto.
+          destruct J0' as [md J0'].
+          rewrite J0'; eauto.
+
+          remember (get_const_metadata c) as R.
+          destruct R as [[[bc ec] tc]|]; eauto.
+            eapply get_const_metadata_isnt_stuck in J0; eauto.
+            destruct J0 as [gvb [gve [Hc1 Hc2]]].
+            rewrite Hc1. rewrite Hc2. simpl.
+            eauto.
+      destruct J2 as [[md0 mt0] J2].
+      assert (exists omd, SBopsem.get_reg_metadata (los, nts) M gl rm v1 = 
+          Some omd) as J3.
+        clear - Hwfm J1 HbInF Hwfc HeqR0. 
+        destruct v1; simpl in *.
+          assert (exists md, lookupAL metadata rm i1 = Some md) as J0'.
+            destruct t; try solve [inversion HeqR0].
+            eapply Hwfm with (t1:=t); eauto.
+              inv Hwfc. inv H12; auto.
+          destruct J0' as [md J0'].
+          rewrite J0'; eauto.
+
+          remember (get_const_metadata c) as R.
+          destruct R as [[[bc ec] tc]|]; eauto.
+            eapply get_const_metadata_isnt_stuck in J1; eauto.
+            destruct J1 as [gvb [gve [Hc1 Hc2]]].
+            rewrite Hc1. rewrite Hc2. simpl.
+            eauto.
+      destruct J3 as [[md1 mt1] J3].
+      remember (if isGVZero (los, nts) gv then 
+                  prop_reg_metadata lc rm i0 gv1 md1
+                else
+                  prop_reg_metadata lc rm i0 gv0 md0) as R.
+      destruct R as [lc' rm'].
+      exists 
+         {|
+         CurSystem := s;
+         CurTargetData := (los, nts);
+         CurProducts := ps;
+         ECS := {|
+                CurFunction := f;
+                CurBB := block_intro l1 ps1
+                           (cs1 ++ insn_select i0 v t v0 v1 :: cs) tmn;
+                CurCmds := cs;
+                Terminator := tmn;
+                Locals := lc';
+                Rmap := rm';
+                Allocas := als |} :: ecs;
+         Globals := gl;
+         FunTable := fs;
+         Mem := M;
+         Mmap := Mmap0 |}.
+       exists trace_nil. eauto.
+
+    SSCase "select_ptr".
+      exists 
+         {|
+         CurSystem := s;
+         CurTargetData := (los, nts);
+         CurProducts := ps;
+         ECS := {|
+                CurFunction := f;
+                CurBB := block_intro l1 ps1
+                           (cs1 ++ insn_select i0 v t v0 v1 :: cs) tmn;
+                CurCmds := cs;
+                Terminator := tmn;
+                Locals := (if isGVZero (los, nts) gv 
+                           then updateAddAL _ lc i0 gv1 
+                           else updateAddAL _ lc i0 gv0);
+                Rmap := rm;
+                Allocas := als |} :: ecs;
+         Globals := gl;
+         FunTable := fs;
+         Mem := M;
+         Mmap := Mmap0 |}.
+       exists trace_nil. eauto.
+
+  SCase "call". 
+    remember (lookupFdefViaGV (los, nts) M ps gl lc fs v) as Hlk. 
+    destruct Hlk as [f' |].
+    SSCase "internal call".
+    assert (exists gvs, params2GVs (los, nts) M p lc gl rm = Some gvs) as G.
+      eapply params2GVs_isnt_stuck; eauto. 
+        exists nil. auto.
+    destruct G as [gvs G].
+    destruct f' as [[fa rt fid la va] lb].
+    assert (J:=HeqHlk).
+    symmetry in HeqHlk.
+    apply lookupFdefViaGV_inv in HeqHlk; auto.
+    eapply wf_system__wf_fdef in HeqHlk; eauto.
+    inv HeqHlk. destruct block5 as [l5 ps5 cs5 tmn5].
+    left.
+    remember (initLocals la gvs rm) as R.
+    destruct R as [lc' rm'].
+    exists 
+         {|
+         CurSystem := s;
+         CurTargetData := (los, nts);
+         CurProducts := ps;
+         ECS :=(mkEC (fdef_intro (fheader_intro fa rt fid la va) lb) 
+                       (block_intro l5 ps5 cs5 tmn5) cs5 tmn5 
+                       lc' rm'
+                       nil)::
+               {|
+                CurFunction := f;
+                CurBB := block_intro l1 ps1
+                           (cs1 ++ insn_call i0 n c t v p :: cs) tmn;
+                CurCmds := insn_call i0 n c t v p :: cs;
+                Terminator := tmn;
+                Locals := lc;
+                Rmap := rm;
+                Allocas := als |} :: ecs;
+         Globals := gl;
+         FunTable := fs;
+         Mem := M;
+         Mmap := Mmap0 |}.
+    exists trace_nil.
+    eauto.    
+
+    remember (lookupExFdecViaGV (los, nts) M ps gl lc fs v) as Helk. 
+    destruct Helk as [f' |].
+    SSCase "external call".
+    assert (exists gvs, LLVMgv.params2GVs (los, nts) M p lc gl = Some gvs) 
+      as G.
+      eapply ssa_wf.params2GVs_isnt_stuck; eauto. 
+        exists nil. auto.
+    destruct G as [gvs G].
+    destruct f' as [[fa rt fid la va]].
+    remember (callExternalFunction M fid gvs) as R.
+    destruct R as [oresult Mem'].
+    remember (exCallUpdateLocals t n i0 oresult lc rm) as R'.
+    destruct R' as [[lc' rm']|].
+      left.
+      exists 
+         {|
+         CurSystem := s;
+         CurTargetData := (los, nts);
+         CurProducts := ps;
+         ECS :={|
+                CurFunction := f;
+                CurBB := block_intro l1 ps1
+                           (cs1 ++ insn_call i0 n c t v p :: cs) tmn;
+                CurCmds := cs;
+                Terminator := tmn;
+                Locals := lc';
+                Rmap := rm';
+                Allocas := als |} :: ecs;
+         Globals := gl;
+         FunTable := fs;
+         Mem := Mem';
+         Mmap := Mmap0 |}.
+      exists trace_nil.
+      eauto.
+
+      right.
+      unfold undefined_state.
+      right. rewrite <- HeqHlk. rewrite <- HeqHelk. rewrite G. rewrite <- HeqR0.
+      rewrite <- HeqR'. undefbehave.
+
+    SSCase "stuck".
+      right.
+      unfold undefined_state.
+      right. rewrite <- HeqHlk. rewrite <- HeqHelk. undefbehave.
+Qed.
+
 
 (*****************************)
 (*
